multiset/IndependenceCommon.v
@@ -2,46 +2,30 @@ Require Import erasure.
 
 Axiom uniqueTP : forall T1 T2 t, tIn (tUnion T1 T2) t -> tIn T1 t -> tIn T2 t -> False. 
 
-Theorem unionEq : forall T1 T2 T2', tUnion T1 T2 = tUnion T1 T2' -> T2 = T2'.  
-Proof.
-  intros. apply Extensionality_Ensembles. unfold Same_set. unfold Included. split; intros. 
-  {apply eqImpliesSameSet in H. unfold Same_set in H. unfold Included in H. inv H. 
-   assert(tIn (tUnion T1 T2) x). apply Union_intror. auto. copy H. apply H1 in H.
-   inversion H; subst. eapply uniqueTP in H0; eauto. inversion H0. auto. }
-  {apply eqImpliesSameSet in H. unfold Same_set in H. unfold Included in H. inv H. 
-   assert(tIn (tUnion T1 T2') x). apply Union_intror. auto. copy H. apply H2 in H3. 
-   inversion H3; subst. eapply uniqueTP in H0; eauto. inversion H0. auto. }
-Qed. 
-
 Theorem UnionEqTID : forall T T' tid s1 s2 M s1' s2' M',
                        tUnion T (tSingleton(tid,s1,s2,M)) = tUnion T' (tSingleton(tid,s1',s2',M')) ->
                        T = T' /\ s1 = s1' /\ s2 = s2' /\ M = M'. 
 Proof. 
-  intros. unfoldSetEq H. assert(tIn (tUnion T (tSingleton(tid,s1,s2,M)))(tid,s1,s2,M)). 
-  apply Union_intror. constructor. copy H.  apply H0 in H. inversion H.  
-  {assert(thread_lookup (tUnion T' (tSingleton(tid,s1',s2',M'))) tid (tid,s1,s2,M)). 
-   econstructor. econstructor. eauto. auto. 
-   assert(thread_lookup (tUnion T' (tSingleton(tid,s1',s2',M'))) tid (tid,s1',s2',M')). 
-   econstructor. apply Union_intror. constructor. auto. eapply uniqueThreadPool in H5; eauto. 
-   inv H5. repeat constructor; auto. eqSets. 
-   {assert(tIn (tUnion T (tSingleton(tid,s1,s2,M))) x). constructor. auto. copy H5. apply H0 in H5. 
-    inversion H5; subst. auto. inv H8. exfalso. eapply uniqueTP; eauto. constructor. }
-   {assert(tIn (tUnion T' (tSingleton(tid,s1,s2,M))) x). constructor. auto. copy H5. 
-    apply H1 in H5. inversion H5; subst. auto. inv H8. exfalso. eapply uniqueTP; eauto. 
-    constructor. }
-  }
-  {subst. inv H3. repeat constructor; auto. eqSets. 
-   {assert(tIn (tUnion T (tSingleton(tid,s1,s2,M))) x). constructor. auto. copy H4. apply H0 in H4. 
-    inversion H4; subst. auto. inv H6. exfalso. eapply uniqueTP; eauto. constructor. }
-   {assert(tIn (tUnion T' (tSingleton(tid,s1,s2,M))) x). constructor. auto. copy H4. 
-    apply H1 in H4. inversion H4; subst. auto. inv H6. exfalso. eapply uniqueTP; eauto. 
-    constructor. }
-  }
+  intros.
+  assert(thread_lookup (tUnion T' (tSingleton(tid,s1',s2',M'))) tid (tid,s1,s2,M)). 
+  econstructor. rewrite <- H. unfoldTac; invUnion. right. simpl; auto. 
+  auto. assert(thread_lookup (tUnion T' (tSingleton(tid,s1',s2',M'))) tid (tid,s1',s2',M')). 
+  econstructor; auto. unfoldTac; invUnion. right; simpl; auto. 
+  eapply uniqueThreadPool in H0; eauto. inv H0. apply UnionEqL in H. subst; auto. 
 Qed. 
 
-Axiom UnionSingletonEq : forall T T' a b, 
+
+
+
+Theorem UnionSingletonEq : forall T T' a b, 
                  tUnion T (tSingleton a) = tUnion T' (tSingleton b) -> 
-                 tIn T' a -> T = tUnion (Subtract thread T' a) (tSingleton b).
+                 tIn T' a -> T = tUnion (Subtract T' a) (tSingleton b).
+Proof.
+  intros. unfoldTac. apply pullOut in H0. rewrite H0 in H. 
+  rewrite <- Union_associative in H.
+  rewrite (Union_commutative thread (Single a)) in H. rewrite Union_associative in H. 
+  apply UnionEqL in H. auto. 
+Qed. 
 
 Ltac proveUnionEq H := apply UnionSingletonEq in H;[rewrite H; unfoldTac; rewrite UnionSwap; auto|idtac]; auto.
 Theorem neqSym : forall (T:Type) (x y : T), x <> y <-> y <> x. 
@@ -57,16 +41,39 @@ Inductive eraseTrm : list action -> trm -> trm -> Prop :=
 |eraseTrmFork : forall t E M d N s n, eraseTrm (s++[fAct t E M d n]) N t
 |eraseTrmSR : forall t E M N d M' s, eraseTrm (s++[srAct t E M N d]) M' t. 
 
+Theorem getLastApp : forall (T:Type) a c (b:T),
+                       last(a++[b]) c = b.
+Proof.
+  induction a; intros. 
+  {simpl. auto. }
+  {simpl. destruct (a0++[b]) eqn:eq. 
+   {invertListNeq. }
+   {rewrite <- eq. eauto. }
+  }
+Qed. 
+
+Theorem unspecLastAct : forall tid s a s2 M' M, 
+                         actionTerm a M' ->
+                         unspecThread(tid,unlocked(s++[a]),s2,M) = tSingleton (tid,unlocked nil,s2,M'). 
+Proof.
+  induction s; intros. 
+  {simpl. inv H; auto. }
+  {simpl. destruct (s++[a0])eqn:eq. 
+   {invertListNeq. }
+   {rewrite <- eq. rewrite getLastApp. inv H; auto. }
+  }
+Qed. 
+
 Theorem unspecEraseTrm : forall tid s1 s2 M M', 
                           eraseTrm s1 M M' ->
-                          unspecThread(tid,unlocked s1,s2,M) (tSingleton(tid,unlocked nil,s2,M')). 
+                          unspecThread(tid,unlocked s1,s2,M) = (tSingleton(tid,unlocked nil,s2,M')). 
 Proof.
   intros. destructLast s1. 
    {inv H; try invertListNeq. auto. }
    {invertHyp. inv H; try solve[invertListNeq]; apply lastElementEq in H1;
-   subst; unspecThreadTac; auto. }
+               subst; erewrite unspecLastAct; eauto; constructor. }
 Qed. 
-
+ 
 Theorem eEraseTrm : forall s1 M, exists M', eraseTrm s1 M M'. 
   intros. destructLast s1. 
   {econstructor. econstructor. }
@@ -96,31 +103,21 @@ Ltac falseDecomp :=
              inv F2
   end. 
 
-Theorem subtractSingle : forall X T x1, 
-              (Subtract X (Union X (Subtract X T x1) (Singleton X x1)) x1) =
-              Subtract X T x1. 
-Proof.
-  intros. eqSets. 
-  {inv H. inv H0. auto. inv H. exfalso. apply H1. constructor. }
-  {inv H. constructor. constructor. constructor. auto. auto. auto. }
-Qed. 
-
-
 Theorem specStepFullIVar' : forall x H H' ds TID s1 s2 N S tid M T t' sc,
        spec_step H T (tSingleton(TID,s1,s2,N)) H' T t' ->
        heap_lookup x H = Some (sfull sc ds S tid M) ->
        (heap_lookup x H' = Some (sfull sc ds S tid M) \/
         heap_lookup x H' = Some(sfull sc (TID::ds) S tid M)). 
 Proof.
-  intros. inv H0; unfoldTac; invertHyp; invThreadEq; eauto. 
+  intros. inv H0; eauto. 
   {destruct (beq_nat x x0) eqn:eq. 
-   {apply beq_nat_true in eq. subst. rewrite H3 in H1. inv H1. 
+   {apply beq_nat_true in eq. subst. rewrite H11 in H1. inv H1. 
     right. erewrite HeapLookupReplace; eauto. }
    {rewrite lookupReplaceNeq. eauto. intros c. subst. apply beq_nat_false in eq. apply eq. 
     auto. }
   }
   {destruct (beq_nat x x0) eqn:eq. 
-   {apply beq_nat_true in eq. subst. rewrite H3 in H1. inv H1. }
+   {apply beq_nat_true in eq. subst. heapsDisagree. }
    {apply beq_nat_false in eq. rewrite lookupReplaceNeq; auto. }
   }
   {destruct H; simpl in *. destruct h. 
@@ -135,14 +132,7 @@ Ltac startIndCase :=
     |H:spec_step ?a ?b ?c ?d ?e ?f,H':tUnion ?T ?t = tUnion ?T' ?t' |- _ =>
      let n := fresh
      in let n' := fresh
-        in copyAs H n; copyAs H' n'; apply specStepSingleton in n; invertHyp;
-           unfoldSetEq n'
-  end. 
-Ltac eqIn H := 
-  match type of H with
-      |forall x, Ensembles.In ?X (tUnion ?T (tSingleton ?x1)) x -> ?a => 
-       let n := fresh 
-       in assert(n:Ensembles.In X (tUnion T (tSingleton x1)) x1) by (apply Union_intror; constructor);apply H in n
+        in copyAs H n; copyAs H' n'; apply specStepSingleton in n; invertHyp
   end. 
 
 Ltac takeTStep :=
@@ -162,17 +152,43 @@ Ltac lookupTac :=
      assert(heap_lookup x' (replace x v H) = Some v') by (rewrite lookupReplaceNeq; auto)
     |H:spec_step ?H ?T ?t (replace ?x ?v ?H) ?T' ?t',H':heap_lookup ?x ?H = Some ?v' |- _ =>
      assert(heap_lookup x (replace x v H) = Some v) by (erewrite HeapLookupReplace; eauto)                             
-    |H:spec_step ?H ?T ?t (extend ?x ?v ?H ?p) ?T' ?t',H':heap_lookup ?x' ?H = Some ?v',H'':?x'<>?x |- _ => 
-     assert(heap_lookup x' (extend x v H p) = Some v') by (apply lookupExtendNeq; eauto)
+    |H:spec_step ?H ?T ?t (Heap.extend ?x ?v ?H ?p) ?T' ?t',H':heap_lookup ?x' ?H = Some ?v',H'':?x'<>?x |- _ => 
+     assert(heap_lookup x' (Heap.extend x v H p) = Some v') by (apply lookupExtendNeq; eauto)
   end. 
 
+
+Ltac destructThread x :=
+     let n1 := fresh in
+     let n2 := fresh in 
+     destruct x as [n1 n2];
+       let n3 := fresh in
+       let n4 := fresh in
+       destruct n1 as [n3 n4];
+         let n5 := fresh in
+         let n6 := fresh in 
+         destruct n3 as [n5 n6]. 
+
 Ltac nonEmptyStackTac H :=
-  eapply nonEmptyStack in H;
-  [ idtac
-  | apply InL; constructor
-  | solveSet
-  | simpl; try rewrite app_nil_l; eauto   
-  | simpl; eauto]. 
+  eapply nonEmptyStack in H;unfoldTac; [idtac|solveSet|solveSet|rewrite app_nil_l; simpl;auto|
+                                        simpl;auto].
+
+Theorem UnionNeqTID : forall T T' tid tid' s1 s2 s1' s2' M M',
+       tUnion T (tSingleton (tid, s1, s2, M)) =
+       tUnion T' (tSingleton (tid', s1', s2', M')) -> tid <> tid' ->
+       T = tUnion (Subtract T' (tid,s1,s2,M)) (tSingleton(tid',s1',s2',M')) /\
+       T' = tUnion (Subtract T (tid',s1',s2',M')) (tSingleton(tid,s1,s2,M)).
+Proof.
+  intros. assert(tIn (tUnion T (tSingleton(tid,s1,s2,M))) (tid',s1',s2',M')). 
+  rewrite H. unfoldTac; invUnion. right; simpl; auto. 
+  assert(tIn (tUnion T' (tSingleton(tid',s1',s2',M'))) (tid,s1,s2,M)). 
+  rewrite <- H. unfoldTac. repeat invUnion. right. simpl; auto. unfoldTac. 
+  repeat invUnion. inv H1; inv H2. 
+  {split. apply UnionSingletonEq in H; auto. symmetry in H. 
+   apply UnionSingletonEq in H; auto. }
+  {inv H1. invThreadEq. exfalso. apply H0. auto. inv H2. }
+  {inv H3; try contradiction. invThreadEq. exfalso. apply H0; auto. }
+  {inv H1; try contradiction. invThreadEq. exfalso. apply H0; auto. }
+Qed. 
 
 Theorem stackNonNil : forall s1 a s1' s2 x M M' tid H H' T T' z,
         eraseTrm (s1'++[x]) z M' ->
@@ -183,33 +199,28 @@ Proof.
   intros. dependent induction H1.  
   {inv H0; invertListNeq; apply app_inj_tail in H1; invertHyp; apply UnionEqTID in x; 
    invertHyp; inv H; exfalso; apply H2; auto. }
-  {copy x. copy H. apply specStepSingleton in H4. invertHyp. unfoldSetEq H3. 
-   assert(tIn (tUnion T0 (tSingleton x1)) x1). apply Union_intror. constructor. 
-   apply H4 in H3. inv H3. 
-   {eapply IHspec_multistep; eauto. apply UnionSingletonEq in x. rewrite x. 
-    unfoldTac. rewrite UnionSwap. auto. auto. }
-   {inv H6. apply eraseTrmApp in H0. inv H0. 
-    {inv H; unfoldTac; invertHyp; invThreadEq; try solve[falseDecomp]. 
-     {inv H3; falseDecomp. }
-     {simpl in *. nonEmptyStackTac H1. invertHyp. introsInv. invertListNeq. }
-    }
-    {inv H; unfoldTac; invertHyp; invThreadEq; try solve[falseDecomp]. 
-     {inv H3; falseDecomp. }
-     {simpl in *. nonEmptyStackTac H1. invertHyp. introsInv. invertListNeq. }
-    }
-    {inv H; unfoldTac; invertHyp; invThreadEq; try solve[falseDecomp]. 
-     {inv H3; falseDecomp. }
-     {simpl in *. nonEmptyStackTac H1. invertHyp. introsInv. invertListNeq. }
-    }
-    {inv H; unfoldTac; invertHyp; invThreadEq; try solve[falseDecomp]. 
-     {inv H3; falseDecomp. }
-     {simpl in *. nonEmptyStackTac H1. invertHyp. introsInv. invertListNeq. }
-    }
-    {inv H; unfoldTac; invertHyp; invThreadEq; try solve[falseDecomp]. 
-     {inv H3; falseDecomp. }
-     {simpl in *. nonEmptyStackTac H1. invertHyp. introsInv. invertListNeq. }
-    }
+  {copy x. copy H. apply specStepSingleton in H4. invertHyp. destructThread x1. 
+   exMid tid H8. 
+   {apply UnionEqTID in H3. invertHyp. apply eraseTrmApp in H0. inv H. 
+    {inv H0; inv H13; falseDecomp. }
+    {inv H0; clear d1; try solve[falseDecomp]. copy d. copy d0. 
+     eapply uniqueCtxtDecomp in H; eauto. invertHyp. nonEmptyStackTac H1.
+     invertHyp. introsInv. invertListNeq. }
+    {inv H0; clear d1; try solve[falseDecomp]. copy d. copy d0. 
+     eapply uniqueCtxtDecomp in H; eauto. invertHyp. nonEmptyStackTac H1.
+     invertHyp. introsInv. invertListNeq. }
+    {inv H0; clear d1; try solve[falseDecomp]. copy d. copy d0. 
+     eapply uniqueCtxtDecomp in H; eauto. invertHyp. nonEmptyStackTac H1.
+     invertHyp. introsInv. invertListNeq. }
+    {inv H0; clear d1; try solve[falseDecomp]. copy d. copy d0. 
+     eapply uniqueCtxtDecomp in H; eauto. invertHyp. nonEmptyStackTac H1.
+     invertHyp. introsInv. invertListNeq. }
+    {inv H0; clear d1; try solve[falseDecomp]. copy d. copy d0. 
+     eapply uniqueCtxtDecomp in H; eauto. invertHyp. nonEmptyStackTac H1.
+     invertHyp. introsInv. invertListNeq. }
    }
+   {apply UnionNeqTID in H3; auto. invertHyp. eapply IHspec_multistep. 
+    eauto. Focus 2. auto. rewrite H4. unfoldTac. rewrite UnionSwap. eauto. auto. }
   }
 Qed. 
 
@@ -222,18 +233,19 @@ Qed.
 
 Ltac proofsEq p p' := assert(p = p') by apply proof_irrelevance; subst. 
 Ltac consedActTac H :=
-  eapply consedActEq in H;[idtac|apply Union_intror; rewrite app_nil_l; constructor|apply Union_intror; constructor].
+  eapply consedActEq in H;[idtac|solveSet|solveSet].
 
 
 Ltac varsEq a b := let n := fresh 
                     in destruct (beq_nat a b) eqn:n;[apply beq_nat_true in n; subst|apply beq_nat_false in n]. 
 
-Ltac flipCouples :=
-  rewrite couple_swap; rewrite coupleUnion; try flipCouples; rewrite <- coupleUnion. 
-
-Ltac flipCouplesIn H :=
-  rewrite couple_swap in H; rewrite coupleUnion in H; try flipCouplesIn H; rewrite <- coupleUnion in H. 
-
-Axiom UnionSingletonCoupleEq : forall T T' a b c, 
+Theorem UnionSingletonCoupleEq : forall T T' a b c, 
                  tUnion T (tSingleton a) = tUnion T' (tCouple b c) -> 
-                 tIn T' a -> T = tUnion (Subtract thread T' a) (tCouple b c).
+                  tIn T' a -> T = tUnion (Subtract T' a) (tCouple b c).
+Proof. 
+  intros. unfoldTac. apply pullOut in H0. rewrite H0 in H. 
+  rewrite <- Union_associative in H. rewrite (Union_commutative thread (Single a)) in H. 
+  rewrite Union_associative in H. apply UnionEqL in H. auto. 
+Qed. 
+
+
