multiset/ReadIndependence.v
@@ -1,6 +1,5 @@
 Require Import erasure. 
 Require Import IndependenceCommon. 
-Require Import Coq.Logic.Classical. 
 
 Theorem readFastForward : forall H T H' T' ds TID x M' E t0 s2 d s1' M N,
          heap_lookup x H = Some(sfull COMMIT ds COMMIT t0 N) ->
@@ -18,39 +17,30 @@ Theorem readFastForward : forall H T H' T' ds TID x M' E t0 s2 d s1' M N,
 Proof.
   intros. genDeps{ds; t0; N}. dependent induction H3; intros. 
   {apply UnionEqTID in x. invertHyp. inv H3. invertListNeq. }
-  {startIndCase. eqIn H5. inv H6.  
-   {copy H0. destruct x1. destruct p. destruct p. eapply specStepFullIVar' in H6; eauto. inv H6. 
-    {eapply IHspec_multistep in H9; eauto. invertHyp. Focus 2. proveUnionEq x. exists x1.
-     exists x2. split. apply pullOut in H8. rewrite H8. unfoldTac. rewrite UnionSwap. 
-     econstructor. eapply specStepChangeUnused. eassumption. unfoldTac. rewrite <- UnionSwap. 
-     eassumption. split. eassumption. exists x3. split. apply pullOut in H8. rewrite H8. 
-     econstructor. eapply specStepChangeUnused. eauto. eauto. eauto. }
-    {assert(t1=TID \/ t1 <> TID). apply classic. inv H6. 
-     {apply UnionEqTID in x. invertHyp. 
-      exists (replace x0 (sfull COMMIT (TID::ds) COMMIT t0 N) H). exists T. split. econstructor. 
-      eapply SGet; eauto. constructor. split. 
-      inversion H0; unfoldTac; invertHyp; invThreadEq; try solve[falseDecomp]. 
-      {inv H10; falseDecomp. }
-      {falseDecomp. rewrite H10 in H2. inv H2. simpl in *. assert(d=d0). apply proof_irrelevance. 
-       subst. eassumption. }
-      exists ds. split. rewrite replaceOverwrite. rewrite replaceSame; eauto. constructor. 
-      split. erewrite HeapLookupReplace; eauto. assumption. }
-     {eapply IHspec_multistep in H9; eauto. Focus 2. proveUnionEq x. invertHyp. 
-      exists x1. exists x2. split. apply pullOut in H8. rewrite H8. unfoldTac. rewrite UnionSwap. 
-      econstructor. eapply specStepChangeUnused. eassumption. unfoldTac. rewrite <- UnionSwap. 
-      eassumption. split. eassumption. exists x3. split. apply pullOut in H8. 
-      rewrite H8. econstructor. eapply specStepChangeUnused. eauto. eauto. split. 
-      eauto. auto. intros c. inv c. apply H10; auto. contradiction. }
-    }
+  {startIndCase. destructThread x1. exMid TID H10. 
+   {apply UnionEqTID in x. invertHyp. econstructor. econstructor. split. econstructor. 
+    eapply SGet; eauto. constructor. split. inv H0; try solve[falseDecomp]. 
+    {inv H16; falseDecomp. }
+    {copy d; copy d0. eapply uniqueCtxtDecomp in H0; eauto. invertHyp. inv H8. 
+     proofsEq d d0. rewrite H16 in H2. inv H2. eauto. }
+    {exists ds. split. rewrite replaceOverwrite. rewrite replaceSame; eauto. 
+     constructor. erewrite HeapLookupReplace; eauto. }
    }
-   {inv H8. exists (replace x0 (sfull COMMIT (TID::ds) COMMIT t0 N) H). exists T. 
-    split. econstructor. eapply SGet; eauto. constructor. split.
-    inv H0; unfoldTac; invertHyp; invThreadEq; try solve[falseDecomp]. 
-    {inv H8; falseDecomp. }
-    {falseDecomp. rewrite H8 in H2. inv H2. apply UnionEqTID in x. invertHyp. simpl in *. 
-     assert(d=d0). apply proof_irrelevance. subst. eassumption. }
-    exists ds. split. rewrite replaceOverwrite. rewrite replaceSame; eauto. 
-    constructor. erewrite HeapLookupReplace; eauto. }
+   {copy H0. eapply specStepFullIVar' in H5; eauto. inv H5. 
+    {eapply IHspec_multistep in H12; eauto. invertHyp. apply UnionNeqTID in x. invertHyp. 
+     exists x1. exists x2. split. rewrite H17. unfoldTac. rewrite UnionSwap. 
+     econstructor. eapply specStepChangeUnused. eassumption. unfoldTac. rewrite UnionSwap. 
+     eassumption. split. eassumption. exists x3. split. rewrite H17. econstructor.
+     eapply specStepChangeUnused. eauto. eauto. eauto. auto. apply UnionNeqTID in x. 
+     invertHyp. rewrite H5. rewrite UnionSubtract. unfoldTac. rewrite UnionSwap; auto. auto. }
+     {eapply IHspec_multistep in H12; eauto. apply UnionNeqTID in x; auto. invertHyp. 
+      exists x1. exists x2. split. rewrite H17. unfoldTac. rewrite UnionSwap. 
+      econstructor. eapply specStepChangeUnused. eassumption. unfoldTac. rewrite <- UnionSwap. 
+      eassumption. split. eassumption. exists x3. split. rewrite H17. econstructor. 
+      eapply specStepChangeUnused. eauto. eauto. split. 
+      eauto. auto. apply UnionNeqTID in x. invertHyp. rewrite H5. rewrite UnionSubtract. 
+      unfoldTac. rewrite UnionSwap. eauto. auto. introsInv. apply H8; auto. contradiction. }
+   }
   }
 Qed. 
 
@@ -64,14 +54,14 @@ Proof.
   {copy H. apply specStepSingleton in H3. invertHyp. destruct x0. destruct p. 
    destruct p. copy H. eapply specStepFullIVar' in H; eauto. inv H. 
    {eapply IHspec_multistep in H4; eauto. }
-   {inv H3; unfoldTac; invertHyp; invThreadEq. 
+   {inv H3.
     {rewrite H4 in H0. inversion H0; invertListNeq. }
     {rewrite H4 in H0. inversion H0; invertListNeq. }
     {destruct (beq_nat x0 x) eqn:eq. apply beq_nat_true in eq. subst.
      eapply IHspec_multistep in H4. invertHyp. exists (x0++[t1]). rewrite <- app_assoc.  
      simpl. eauto. eauto. apply beq_nat_false in eq. rewrite lookupReplaceNeq in H4; auto. 
      rewrite H4 in H0. inversion H0; invertListNeq. }
-    {destruct (beq_nat x0 x) eqn:eq. apply beq_nat_true in eq. subst. rewrite H5 in H0. 
+    {destruct (beq_nat x0 x) eqn:eq. apply beq_nat_true in eq. subst. rewrite H13 in H0. 
      inv H0. apply beq_nat_false in eq. rewrite lookupReplaceNeq in H4; eauto. rewrite H4 in H0. 
      inversion H0. invertListNeq. }
     {destruct (beq_nat x0 x) eqn:eq. apply beq_nat_true in eq. subst. copy p. rewrite H in H0. 
@@ -81,93 +71,6 @@ Proof.
    }
   }
 Qed. 
-
-
-
-
-Theorem readSimPureSteps : forall H T H' T' TID x M' t0 E M'' d N N' N'' s2 s1' ds1 ds1' ds2,
-       eraseTrm s1' N' N'' -> 
-       heap_lookup x H = Some(sfull COMMIT (ds1++[TID]++ds2) COMMIT t0 M'') ->       
-       heap_lookup x H' = Some(sfull COMMIT (ds1'++[TID]++ds2) COMMIT t0 M'') -> 
-       spec_multistep H (tUnion T (tSingleton(TID,unlocked[rAct x M' E d],s2,N))) H'
-                      (tUnion T' (tSingleton(TID,unlocked(s1'++[rAct x M' E d]),s2,N'))) ->
-       exists H'' T'',
-         spec_multistep H (tUnion T (tSingleton(TID,unlocked[rAct x M' E d],s2,N))) 
-                        H'' (tUnion T'' (tSingleton(TID,unlocked[rAct x M' E d],s2,N''))) /\
-         spec_multistep H'' (tUnion T'' (tSingleton(TID,unlocked[rAct x M' E d],s2,N''))) 
-                        H' (tUnion T' (tSingleton(TID,unlocked(s1'++[rAct x M' E d]),s2,N'))) /\
-         exists ds1'',
-         spec_multistep (replace x (sfull COMMIT (ds1++ds2) COMMIT t0 M'') H) T 
-                        (replace x (sfull COMMIT (ds1''++ds2) COMMIT t0 M'')H'') T'' /\
-         heap_lookup x H'' = Some(sfull COMMIT (ds1''++[TID]++ds2) COMMIT t0 M'').
-Proof.
-  intros. genDeps{ds1;ds2;t0;M'';ds1'}. dependent induction H3; intros. 
-  {apply UnionEqTID in x. invertHyp. rewrite H2 in H1. inv H1. inv H. 
-   destruct s1'; inv H4. inv H0; try solve[invertListNeq]. exists H'. exists T'. 
-   split. constructor. split. constructor. exists ds1. split. constructor. 
-   apply app_inv_tail in H5. subst. auto. invertListNeq. }
-  {startIndCase. eqIn H5. inv H6. 
-   {copy H1. clear H1. inversion H6; subst; unfoldTac; invertHyp. 
-    {eapply IHspec_multistep in H4;[idtac|eauto|eauto|eauto|eauto|eauto|eauto]. Focus 2.
-     proveUnionEq x. invertHyp. econstructor. econstructor. split. takeTStep. eassumption. 
-     split. eassumption. econstructor. split. apply pullOut in H8. rewrite H8. 
-     econstructor. eapply SBasicStep; eauto. eassumption. eauto. }
-    {eapply IHspec_multistep in H4;[idtac|eauto|eauto|eauto|eauto|eauto|eauto]. Focus 2.
-     proveUnionEq x. invertHyp. econstructor. econstructor. split. takeTStep. eassumption. 
-     split. eassumption. econstructor. split. apply pullOut in H8. rewrite H8. 
-     econstructor. eapply SFork; eauto. eassumption. eauto. }
-    {destruct (beq_nat x2 x0) eqn:eq. apply beq_nat_true in eq. subst. lookupTac. 
-     rewrite H9 in H4. inv H4. simpl in *. rewrite app_comm_cons in H1.   
-     eapply IHspec_multistep in H1; eauto. Focus 2. proveUnionEq x. invertHyp. 
-     econstructor. econstructor. split. takeTStep. eassumption. split. eassumption. econstructor. 
-     split. apply pullOut in H8. rewrite H8. econstructor. eapply SGet with(x:=x0); eauto. 
-     erewrite HeapLookupReplace; eauto. rewrite replaceOverwrite. rewrite replaceOverwrite in H11. 
-     eassumption. eauto. apply beq_nat_false in eq. apply neqSym in eq. lookupTac. 
-     eapply IHspec_multistep in H1; eauto. Focus 2. proveUnionEq x. invertHyp. econstructor. 
-     econstructor. split. takeTStep. eassumption. split. eassumption. econstructor. split. 
-     apply pullOut in H8; rewrite H8. econstructor. eapply SGet with(x:=x2); eauto. 
-     rewrite lookupReplaceNeq; eauto. rewrite lookupReplaceSwitch. eassumption. auto. 
-     eauto. }
-    {destruct (beq_nat x0 x2)eqn:eq. apply beq_nat_true in eq. subst. rewrite H9 in H4. 
-     inv H4. apply beq_nat_false in eq. lookupTac. eapply IHspec_multistep in H1; eauto. 
-     Focus 2. proveUnionEq x. invertHyp. econstructor. econstructor. split. takeTStep. 
-     eassumption. split. eassumption. econstructor. split. apply pullOut in H8; rewrite H8. 
-     econstructor. eapply SPut with(x:=x2); eauto. rewrite lookupReplaceNeq; eauto. 
-     rewrite lookupReplaceSwitch; eauto. eauto. }
-    {destruct (beq_nat x0 x2) eqn:eq. apply beq_nat_true in eq. subst. copy p. rewrite H1 in H4. 
-     inv H4. apply beq_nat_false in eq. lookupTac. eapply IHspec_multistep in H1; eauto.
-     invertHyp. econstructor. econstructor. split. takeTStep. eauto. split. eauto. 
-     econstructor. split. apply pullOut in H8. rewrite H8. econstructor. eapply SNew with (x:=x2); auto. 
-     erewrite extendReplaceSwitch; eauto. eauto. proveUnionEq x. }
-    {eapply IHspec_multistep in H4;[idtac|eauto|eauto|eauto|eauto|eauto|eauto]. Focus 2.
-     proveUnionEq x. invertHyp. econstructor. econstructor. split. takeTStep. eassumption. 
-     split. eassumption. econstructor. split. apply pullOut in H8. rewrite H8. 
-     econstructor. eapply SSpec; eauto. eauto. eauto. }
-   } 
-   {inv H8. apply UnionEqTID in x. invertHyp. inversion H1; subst; unfoldTac; invertHyp; invThreadEq. 
-    {eapply IHspec_multistep in H4;[idtac|eauto|eauto|eauto|eauto|eauto|eauto]. invertHyp. 
-     econstructor. econstructor. split. econstructor. eapply SBasicStep; eauto. eassumption. 
-     split. eauto. econstructor. split. eauto. eauto. }
-    {copy H3. nonEmptyStackTac H3. invertHyp. apply eraseTrmApp in H0. inv H0. exists h'. exists T. 
-     split. constructor. split. simpl. econstructor. eapply SFork; eauto. eassumption. 
-     econstructor. split. constructor. eauto. }
-    {copy H3. nonEmptyStackTac H3. invertHyp. apply eraseTrmApp in H0. inv H0. exists H. exists T. 
-     split. constructor. split. simpl. econstructor. eapply SGet; eauto. eassumption. 
-     econstructor. split. constructor. eauto. }
-    {copy H3. nonEmptyStackTac H3. invertHyp. apply eraseTrmApp in H0. inv H0. exists H. exists T. 
-     split. constructor. split. simpl. econstructor. eapply SPut; eauto. eassumption. 
-     econstructor. split. constructor. eauto. }
-    {copy H3. nonEmptyStackTac H3. invertHyp. apply eraseTrmApp in H0. inv H0. exists H. exists T. 
-     split. constructor. split. simpl. econstructor. eapply SNew; eauto. eassumption. 
-     econstructor. split. constructor. eauto. }
-    {copy H3. nonEmptyStackTac H3. invertHyp. apply eraseTrmApp in H0. inv H0. exists h'. exists T. 
-     split. constructor. split. simpl. econstructor. eapply SSpec; eauto. eassumption. 
-     econstructor. split. constructor. eauto. }
-   }
-  }
-  Grab Existential Variables. rewrite lookupReplaceNeq; eauto. 
-Qed. 
-
 
 Theorem stepWithoutReader : forall H T H' T' ds1 ds2 ds1' t t0 N x,
                               heap_lookup x H = Some(sfull COMMIT (ds1 ++ [t]++ds2) COMMIT t0 N) ->
@@ -199,6 +102,66 @@ Proof.
   Grab Existential Variables. rewrite lookupReplaceNeq; eauto.
 Qed. 
 
+Theorem readSimPureSteps : forall H T H' T' TID x M' t0 E M'' d N N' N'' s2 s1' ds1 ds1' ds2,
+       eraseTrm s1' N' N'' -> 
+       heap_lookup x H = Some(sfull COMMIT (ds1++[TID]++ds2) COMMIT t0 M'') ->       
+       heap_lookup x H' = Some(sfull COMMIT (ds1'++[TID]++ds2) COMMIT t0 M'') -> 
+       spec_multistep H (tUnion T (tSingleton(TID,unlocked[rAct x M' E d],s2,N))) H'
+                      (tUnion T' (tSingleton(TID,unlocked(s1'++[rAct x M' E d]),s2,N'))) ->
+       exists H'' T'',
+         spec_multistep H (tUnion T (tSingleton(TID,unlocked[rAct x M' E d],s2,N))) 
+                        H'' (tUnion T'' (tSingleton(TID,unlocked[rAct x M' E d],s2,N''))) /\
+         spec_multistep H'' (tUnion T'' (tSingleton(TID,unlocked[rAct x M' E d],s2,N''))) 
+                        H' (tUnion T' (tSingleton(TID,unlocked(s1'++[rAct x M' E d]),s2,N'))) /\
+         exists ds1'',
+         spec_multistep (replace x (sfull COMMIT (ds1++ds2) COMMIT t0 M'') H) T 
+                        (replace x (sfull COMMIT (ds1''++ds2) COMMIT t0 M'')H'') T'' /\
+         heap_lookup x H'' = Some(sfull COMMIT (ds1''++[TID]++ds2) COMMIT t0 M'').
+Proof.
+  intros. genDeps{ds1;ds2;t0;M'';ds1'}. dependent induction H3; intros. 
+  {apply UnionEqTID in x. invertHyp. rewrite H2 in H1. inv H1. inv H. 
+   destruct s1'; inv H4. inv H0; try solve[invertListNeq]. exists H'. exists T'. 
+   split. constructor. split. constructor. exists ds1. split. constructor. 
+   apply app_inv_tail in H5. subst. auto. invertListNeq. }
+  {startIndCase. destructThread x1. exMid H10 TID. 
+   {apply UnionEqTID in x. invertHyp. inv H1. 
+    {eapply IHspec_multistep in H4;[idtac|eauto|eauto|eauto|eauto|eauto|eauto]. invertHyp. 
+     econstructor. econstructor. split. econstructor. eapply SBasicStep; eauto. eassumption. 
+     split. eauto. econstructor. split. eauto. eauto. }
+    {copy H3. nonEmptyStackTac H3. invertHyp. apply eraseTrmApp in H0. inv H0. exists h'. exists T. 
+     split. constructor. split. simpl. econstructor. eapply SFork; eauto. eassumption. 
+     econstructor. split. constructor. eauto. }
+    {copy H3. nonEmptyStackTac H3. invertHyp. apply eraseTrmApp in H0. inv H0. exists H. exists T. 
+     split. constructor. split. simpl. econstructor. eapply SGet; eauto. eassumption. 
+     econstructor. split. constructor. eauto. }
+    {copy H3. nonEmptyStackTac H3. invertHyp. apply eraseTrmApp in H0. inv H0. exists H. exists T. 
+     split. constructor. split. simpl. econstructor. eapply SPut; eauto. eassumption. 
+     econstructor. split. constructor. eauto. }
+    {copy H3. nonEmptyStackTac H3. invertHyp. apply eraseTrmApp in H0. inv H0. exists H. exists T. 
+     split. constructor. split. simpl. econstructor. eapply SNew; eauto. eassumption. 
+     econstructor. split. constructor. eauto. }
+    {copy H3. nonEmptyStackTac H3. invertHyp. apply eraseTrmApp in H0. inv H0. exists h'. exists T. 
+     split. constructor. split. simpl. econstructor. eapply SSpec; eauto. eassumption. 
+     econstructor. split. constructor. eauto. }
+   }
+   {apply UnionNeqTID in x; auto. invertHyp. copy H1. eapply specStepFullIVar' in H1; eauto. 
+    inversion H1. 
+    {copy H14. eapply IHspec_multistep in H14; eauto. invertHyp. econstructor. econstructor. 
+     split. rewrite H12. unfoldTac. rewrite UnionSwap. econstructor. eapply specStepChangeUnused. 
+     eauto. unfoldTac. rewrite UnionSwap. eassumption. split; eauto. exists x2. split. 
+     eapply spec_multi_trans. Focus 2. eassumption. eapply stepWithoutReader; eauto. 
+     rewrite H12. econstructor. eapply specStepChangeUnused; eauto. constructor. eauto. 
+     rewrite H5. unfoldTac. rewrite UnionSubtract. rewrite UnionSwap. auto. }
+    {copy H14. rewrite app_comm_cons in H14. eapply IHspec_multistep in H14; eauto. invertHyp. 
+     econstructor. econstructor. split. rewrite H12. unfoldTac. rewrite UnionSwap. econstructor. 
+     eapply specStepChangeUnused. eauto. unfoldTac. rewrite UnionSwap. eassumption. split; eauto. 
+     exists x2. split. eapply spec_multi_trans. Focus 2. eassumption. eapply stepWithoutReader; eauto. 
+     rewrite H12. econstructor. eapply specStepChangeUnused; eauto. constructor. eauto. 
+     rewrite H5. unfoldTac. rewrite UnionSubtract. rewrite UnionSwap. auto. }
+   }
+  }
+Qed. 
+
 Theorem readSimActionSteps : forall H T H' T' TID x M' E M'' d N N' t0 H'' T'' N'' s2 s1 s1' ds1 ds1' ds2 a,
        eraseTrm (s1'++[a]) N' N'' ->
        heap_lookup x H = Some(sfull COMMIT (ds1++[TID]++ds2) COMMIT t0 M'') ->       
@@ -217,54 +180,22 @@ Proof.
    replace[a;rAct x0 M' E d] with ([a]++[rAct x0 M' E d]) in H6; auto. 
    rewrite app_assoc in H6. apply app_inj_tail in H6. invertHyp. rewrite H2 in H1. 
    inv H1. apply app_inv_tail in H6. subst. constructor. }
-  {copy x. copy H1. apply specStepSingleton in H1. invertHyp. unfoldSetEq H6.
-   assert(tIn(tUnion T0(tSingleton x1)) x1). apply Union_intror. constructor. 
-   apply H1 in H6. inv H6.  
-   {copy H9. apply pullOut in H9. rewrite H9. clear H9. copy H7. destruct x1. destruct p.  
-    destruct p. copy H9. eapply specStepFullIVar' in H9; eauto. inv H9.  
-    {eapply spec_multi_trans. eapply spec_multi_unused. eapply stepWithoutReader; eauto. 
-     eapply smulti_step. eapply specStepChangeUnused. eassumption. constructor. 
-     eapply IHspec_multistep in H11; eauto. eapply spec_multi_trans. eassumption. 
-     apply pullOut in H6. rewrite H6. unfoldTac. rewrite UnionSwap. econstructor. 
-     eapply specStepChangeUnused. eauto. unfoldTac. rewrite <- UnionSwap. 
-     rewrite subtractSingle. constructor. proveUnionEq x. }
-    {inversion H10; subst; unfoldTac; invertHyp; invThreadEq. 
-     {rewrite H5 in H11. inversion H11. invertListNeq. }
-     {rewrite H5 in H11. inversion H11. invertListNeq. }
-     {destruct (beq_nat x0 x1) eqn:eq. apply beq_nat_true in eq. subst. rewrite H12 in H5. 
-      inv H5. copy H11. repeat rewrite app_comm_cons in H5. eapply IHspec_multistep in H5; eauto.
-      rewrite UnionSwap. econstructor. eapply SGet with(x:=x1); eauto. erewrite HeapLookupReplace; eauto. 
-      rewrite replaceOverwrite. rewrite replaceOverwrite in H5. simpl in *. unfoldTac. 
-      rewrite <- UnionSwap. eassumption. eapply spec_multi_trans. eassumption. apply pullOut in H6.
-      rewrite H6. rewrite UnionSwap. econstructor. eapply SGet with(x:=x1); eauto. 
-      rewrite <- UnionSwap. simpl. rewrite subtractSingle. constructor. proveUnionEq x. 
-      apply beq_nat_false in eq. rewrite lookupReplaceNeq in H11. rewrite H11 in H5. 
-      inversion H5. invertListNeq. auto. }
-     {destruct (beq_nat x0 x1) eqn:eq. apply beq_nat_true in eq. subst. rewrite H12 in H5. 
-      inv H5. rewrite lookupReplaceNeq in H11. rewrite H11 in H5. inversion H5. invertListNeq. 
-      apply beq_nat_false in eq. auto. }
-     {destruct (beq_nat x0 x1) eqn:eq. apply beq_nat_true in eq. subst. copy p. rewrite H9 in H5. 
-      inv H5. apply beq_nat_false in eq. erewrite lookupExtendNeq in H11; eauto. 
-      inversion H11. invertListNeq. }
-     {rewrite H5 in H11. inversion H11. invertListNeq. }
-    }
-   }
-   {inv H9. apply UnionEqTID in x. invertHyp. inv H6. 
-    inversion H7; subst; unfoldTac; invertHyp; invThreadEq.  
+  {startIndCase. destructThread x1. exMid TID H11. 
+   {apply UnionEqTID in x. invertHyp. inversion H1; subst. 
     {copy H3. eapply stackNonNil in H3. destruct s1. exfalso. apply H3. auto. 
      econstructor. eapply SBasicStep; eauto. constructor. eapply IHspec_multistep; eauto. 
      eapply spec_multi_trans. eassumption. econstructor. eapply SBasicStep; eauto. constructor. 
-     eauto. intros c. subst. apply eraseTrmApp in H0. inv H0; inv H10; falseDecomp. }
-    {econstructor. eapply SFork; eauto. unfoldTac. rewrite coupleUnion. rewrite <- Union_associative. 
+     eauto. intros c. subst. apply eraseTrmApp in H0. inv H0; inv H17; falseDecomp. }
+    {econstructor. eapply SFork; eauto. unfoldTac. rewrite coupleUnion. rewrite Union_associative. 
      rewrite <- UnionSwap. eapply IHspec_multistep; eauto. Focus 2. 
-     rewrite Union_associative. rewrite <- coupleUnion. rewrite couple_swap. 
+     rewrite <- Union_associative. rewrite <- coupleUnion. rewrite couple_swap. 
      unfold numForks. simpl. simpl. eauto. rewrite numForksDistribute. simpl. rewrite <- plus_assoc. 
      rewrite <- plus_comm. simpl. rewrite plus_comm. reflexivity. eapply spec_multi_trans. 
-     eassumption. econstructor. eapply SFork; eauto. rewrite Union_associative. rewrite <- coupleUnion. 
+     eassumption. econstructor. eapply SFork; eauto. rewrite <- Union_associative. rewrite <- coupleUnion. 
      rewrite couple_swap. simpl. rewrite numForksDistribute. simpl. rewrite <- plus_assoc. 
      rewrite plus_comm. simpl. rewrite plus_comm. constructor. }
     {destruct(beq_nat x x0) eqn:eq. 
-     {apply beq_nat_true in eq. subst. rewrite H5 in H10. inv H10. econstructor. 
+     {apply beq_nat_true in eq. subst. rewrite H5 in H17. inv H17. econstructor. 
       eapply SGet with(x:=x0); eauto. erewrite HeapLookupReplace; eauto. lookupTac. simpl in *. 
       rewrite app_comm_cons in H6. eapply IHspec_multistep in H6; eauto. rewrite replaceOverwrite. 
       rewrite replaceOverwrite in H6. eassumption. eapply spec_multi_trans. eassumption. econstructor. 
@@ -274,7 +205,7 @@ Proof.
       rewrite lookupReplaceSwitch; auto. eassumption. eapply spec_multi_trans. eassumption. 
       econstructor. eapply SGet with(x:=x); eauto. constructor. simpl. eauto. }
     }
-    {destruct (beq_nat x x0) eqn:eq. apply beq_nat_true in eq. subst. rewrite H10 in H5. 
+    {destruct (beq_nat x x0) eqn:eq. apply beq_nat_true in eq. subst. rewrite H17 in H5. 
      inv H5. apply beq_nat_false in eq. apply neqSym in eq. lookupTac.
      eapply IHspec_multistep in H6; eauto. econstructor. eapply SPut with(x:=x). 
      rewrite lookupReplaceNeq; eauto. auto. rewrite lookupReplaceSwitch; auto. simpl. 
@@ -285,12 +216,31 @@ Proof.
      eapply IHspec_multistep in H6; eauto. econstructor. eapply SNew with(x:=x). 
      auto. erewrite extendReplaceSwitch; eauto. eapply spec_multi_trans. eassumption. 
      econstructor. eapply SNew with(x:=x); eauto. constructor. simpl. auto. }
-    {econstructor. eapply SSpec; eauto. unfoldTac. rewrite coupleUnion. rewrite <- Union_associative. 
-     rewrite <- UnionSwap. eapply IHspec_multistep; eauto. Focus 2. rewrite Union_associative. 
+    {econstructor. eapply SSpec; eauto. unfoldTac. rewrite coupleUnion. rewrite Union_associative. 
+     rewrite <- UnionSwap. eapply IHspec_multistep; eauto. Focus 2. rewrite <- Union_associative. 
      rewrite <- coupleUnion.  rewrite couple_swap. reflexivity. eapply spec_multi_trans. 
-     eassumption. econstructor. eapply SSpec; eauto. rewrite Union_associative. rewrite <- coupleUnion. 
-     rewrite couple_swap. constructor. }
+     eassumption. econstructor. eapply SSpec; eauto. rewrite <- Union_associative. 
+     rewrite <- coupleUnion. rewrite couple_swap. constructor. }
+   }
+   {apply UnionNeqTID in H7; auto. invertHyp. copy H1. eapply specStepFullIVar' in H1; eauto. 
+    inversion H1. 
+    {copy H14. eapply IHspec_multistep in H14; eauto. eapply spec_multi_trans. Focus 2. 
+     eassumption. eapply stepWithoutReader; eauto. rewrite H13. unfoldTac. rewrite UnionSwap. 
+     econstructor. eapply specStepChangeUnused. eauto. unfoldTac. rewrite UnionSwap. 
+     constructor. eapply spec_multi_trans. eassumption. rewrite H13. unfoldTac. 
+     rewrite UnionSwap. econstructor. eapply specStepChangeUnused. eauto. unfoldTac. 
+     rewrite UnionSwap. constructor. rewrite H6. rewrite UnionSubtract. unfoldTac. 
+     rewrite UnionSwap. eauto. }
+    {copy H14. rewrite app_comm_cons in H14. eapply IHspec_multistep in H14; eauto. 
+     eapply spec_multi_trans. Focus 2. 
+     eassumption. eapply stepWithoutReader; eauto. rewrite H13. unfoldTac. rewrite UnionSwap. 
+     econstructor. eapply specStepChangeUnused. eauto. unfoldTac. rewrite UnionSwap. 
+     constructor. eapply spec_multi_trans. eassumption. rewrite H13. unfoldTac. 
+     rewrite UnionSwap. econstructor. eapply specStepChangeUnused. eauto. unfoldTac. 
+     rewrite UnionSwap. constructor. rewrite H6. rewrite UnionSubtract. unfoldTac. 
+     rewrite UnionSwap. eauto. }
    }
   }
   Grab Existential Variables. rewrite lookupReplaceNeq; eauto. 
 Qed. 
+     
