multiset/newIndependence.v
@@ -10,40 +10,40 @@ Theorem newFastForward : forall H T H' T' TID x M' E s2 d s1' p M,
                          (tUnion T'' (tSingleton(TID,unlocked [nAct M' E d x],s2,fill E (ret (fvar x))))) /\
            spec_multistep H'' (tUnion T'' (tSingleton(TID,unlocked [nAct M' E d x],s2,fill E (ret (fvar x)))))
                           H' (tUnion T' (tSingleton(TID,unlocked(s1'++[nAct M' E d x]),s2,M)))  /\
-           spec_multistep (extend x (sempty COMMIT) H p) T 
+           spec_multistep (Heap.extend x (sempty COMMIT) H p) T 
                           (replace x (sempty COMMIT) H'') T'' /\ 
            heap_lookup x H'' = Some(sempty SPEC).
 Proof.
   intros. dependent induction H2. 
   {apply UnionEqTID in x. invertHyp. inv H2. invertListNeq. }
-  {startIndCase. eqIn H4. inv H5. 
-   {copy H3. eapply specStepNoneIVar in H3; eauto. Focus 3. apply Union_intror. constructor.
-    Focus 2. apply UnionSingletonEq in x. rewrite x. constructor. apply Union_intror. constructor. 
-    auto. eapply IHspec_multistep with(p:=H3)in H1. Focus 2. eassumption. Focus 2. auto. Focus 3. auto. 
-    invertHyp. exists x2. exists x3. split. copy H7. apply pullOut in H10. rewrite H10. 
-    unfoldTac. rewrite UnionSwap. econstructor. eapply specStepChangeUnused. eauto. 
-    unfoldTac. rewrite <- UnionSwap. eassumption. split. eassumption. split.
-    apply pullOut in H7. rewrite H7. clear H7. inv H5; unfoldTac; invertHyp.
-    {econstructor. eapply SBasicStep; eauto. proofsEq p H3. eassumption. }
-    {econstructor. eapply SFork. auto. proofsEq p H3. eauto. }
-    {destruct (beq_nat x4 x0) eqn:eq. apply beq_nat_true in eq. subst. rewrite H0 in H10.
-     inv H10. apply beq_nat_false in eq. econstructor. eapply SGet with(x:=x4); auto. 
-     erewrite lookupExtendNeq; eauto. erewrite <- extendReplaceSwitch; eauto. }
-    {destruct (beq_nat x4 x0) eqn:eq. apply beq_nat_true in eq. subst.
-     rewrite H0 in H10. inv H10. apply beq_nat_false in eq. econstructor. eapply SPut with(x:=x4). 
-     erewrite lookupExtendNeq; eauto. auto. erewrite <- extendReplaceSwitch; eauto. }
-    {destruct (beq_nat x4 x0)eqn:eq. apply beq_nat_true in eq. subst. 
-     copy H3. erewrite lookupExtend in H5. inv H5. apply beq_nat_false in eq. 
-     econstructor. eapply SNew with(x:=x4). auto. erewrite extendExtendSwitch. eassumption. }
-    {econstructor. eapply SSpec; eauto. proofsEq p H3. eassumption. }
-    auto. proveUnionEq x.
-   }
-   {inv H7. apply UnionEqTID in x. invertHyp. clear H5 H7 H9. econstructor. 
-    exists T. split. econstructor. eapply SNew with (x:=x0)(p:=p). eauto. simpl. constructor.
-    split. inv H3; unfoldTac; invertHyp; invThreadEq; try solve[falseDecomp]. 
-    {inv H7; falseDecomp. }
+  {startIndCase. destructThread x1. exMid TID H9. 
+   {apply UnionEqTID in H5. invertHyp. econstructor. exists T. split. econstructor. 
+    eapply SNew with (x:=x0)(p:=p). eauto. simpl. constructor.
+    split. inv H3;try solve[falseDecomp]. 
+    {inv H14; falseDecomp. }
     {simpl in *. copy H2. firstActTac H2. inv H2. proofsEq d d0. proofsEq p p0. eassumption. }
     split. erewrite replaceExtendOverwrite. constructor. rewrite lookupExtend. auto. 
+   }
+   {apply UnionNeqTID in x. invertHyp. copy H3. eapply specStepNoneIVar in H3; eauto. 
+    Focus 3. solveSet. Focus 2. rewrite H4. solveSet. left. invUnion. right. simpl; auto. 
+    Focus 2. auto. eapply IHspec_multistep with(p:=H3)in H1. Focus 2. eassumption. 
+    Focus 2. auto. Focus 3. auto. invertHyp. exists x. exists x1. split. rewrite H11. 
+    unfoldTac. rewrite UnionSwap. econstructor. eapply specStepChangeUnused. eauto. 
+    unfoldTac. rewrite <- UnionSwap. eassumption. split. eassumption. split.
+    rewrite H11. clear H11 H4. inv H12. 
+    {econstructor. eapply SBasicStep; eauto. proofsEq p H3. eassumption. }
+    {econstructor. eapply SFork. auto. proofsEq p H3. eauto. }
+    {destruct (beq_nat x2 x0) eqn:eq. apply beq_nat_true in eq. subst. rewrite H0 in H23.
+     inv H23. apply beq_nat_false in eq. econstructor. eapply SGet with(x:=x2); auto. 
+     erewrite lookupExtendNeq; eauto. erewrite <- extendReplaceSwitch; eauto. }
+    {destruct (beq_nat x2 x0) eqn:eq. apply beq_nat_true in eq. subst.
+     rewrite H0 in H23. inv H23. apply beq_nat_false in eq. econstructor. eapply SPut with(x:=x2). 
+     erewrite lookupExtendNeq; eauto. auto. erewrite <- extendReplaceSwitch; eauto. }
+    {destruct (beq_nat x2 x0)eqn:eq. apply beq_nat_true in eq. subst. 
+     copy H3. erewrite lookupExtend in H4. inv H4. apply beq_nat_false in eq. 
+     econstructor. eapply SNew with(x:=x2). auto. erewrite extendExtendSwitch. eassumption. }
+    {econstructor. eapply SSpec; eauto. proofsEq p H3. eassumption. }
+    auto. rewrite H4. rewrite UnionSubtract. unfoldTac. rewrite UnionSwap; eauto. 
    }
   }
   Grab Existential Variables. eapply lookupExtendNeq; eauto.  
@@ -106,15 +106,8 @@ Proof.
   intros. dependent induction H3. 
   {apply UnionEqTID in x. invertHyp. inv H. destruct s1'; inv H5; try invertListNeq. 
    inv H0; try invertListNeq. repeat econstructor. eauto. }
-  {startIndCase. eqIn H5. inv H6. 
-   {copy H4. eapply specStepEmptyIVar' in H4; eauto. copy H4. 
-    eapply IHspec_multistep in H4;[idtac|eauto|idtac|auto|proveUnionEq x|auto|auto].
-    Focus 2. auto. invertHyp. econstructor. econstructor. split. takeTStep. eassumption.  
-    split. assumption. split. Focus 2. auto. eapply stepReplaceEmpty in H6; eauto. 
-    apply pullOut in H8. rewrite H8. econstructor. eapply specStepChangeUnused. eauto. 
-    assumption. }
-   {inv H8. apply UnionEqTID in x. invertHyp. clear H6 H8 H10. 
-    inversion H4; unfoldTac; invertHyp; invThreadEq. 
+  {startIndCase. destructThread x1. exMid H10 TID.
+   {apply UnionEqTID in x. invertHyp. inversion H4; subst. 
     {eapply IHspec_multistep in H1;[idtac|eauto|idtac|auto|auto|auto|auto]; auto. 
      invertHyp. econstructor. econstructor. split. econstructor. eapply SBasicStep; eauto.
      eassumption. split; auto. }
@@ -123,13 +116,14 @@ Proof.
      split. constructor. auto. }
     {copy H3. nonEmptyStackTac H3. invertHyp. apply eraseTrmApp in H0. inv H0. 
      do 4 econstructor. simpl in *. destruct (beq_nat x x0) eqn:eq. apply beq_nat_true in eq.
-     subst. rewrite H8 in H1. inv H1. apply beq_nat_false in eq. econstructor. 
+     subst. rewrite H15 in H1. inv H1. apply beq_nat_false in eq. econstructor. 
      eapply SGet with(x:=x); eauto. simpl in *. eassumption. split. constructor. auto. }
     {copy H3. nonEmptyStackTac H3. invertHyp. apply eraseTrmApp in H0. inv H0. 
      do 4 econstructor. simpl in *. destruct (beq_nat x x0) eqn:eq. apply beq_nat_true in eq.
-     subst. eapply smultiEmptyFull in H6; eauto. contradiction. erewrite HeapLookupReplace; eauto. 
-     rewrite H8 in H1. inv H1. auto. apply beq_nat_false in eq. econstructor. 
-     eapply SPut with(x:=x); eauto. simpl in *. eassumption. split. constructor. auto. }
+     subst. eapply smultiEmptyFull in H5. Focus 3. eauto. Focus 2. rewrite H15 in H1.
+     inv H1. erewrite HeapLookupReplace; eauto. contradiction. 
+     apply beq_nat_false in eq. econstructor. eapply SPut with(x:=x); eauto. simpl in *. 
+     eassumption. split. constructor. auto. }
     {copy H3. nonEmptyStackTac H3. invertHyp. apply eraseTrmApp in H0. inv H0. 
      do 4 econstructor. simpl in *. destruct (beq_nat x x0) eqn:eq. apply beq_nat_true in eq.
      subst. copy p. rewrite H0 in H1. inv H1. apply beq_nat_false in eq. econstructor. 
@@ -138,8 +132,15 @@ Proof.
      do 4 econstructor. econstructor. eapply SSpec; eauto. simpl in *. eassumption. 
      split. constructor. auto. }
    }
+   {apply UnionNeqTID in x; auto. invertHyp. copy H4. eapply specStepEmptyIVar' in H4; eauto. copy H4. 
+    eapply IHspec_multistep in H4;[idtac|eauto|idtac|auto|idtac|auto|auto].
+    Focus 2. auto. invertHyp. econstructor. econstructor. split. rewrite H12. 
+    unfoldTac. rewrite UnionSwap. econstructor. eapply specStepChangeUnused; eauto.
+    unfoldTac. rewrite UnionSwap. eauto. split; auto. split. rewrite H12. 
+    econstructor. eapply stepReplaceEmpty. eauto. eapply H14.  eapply specStepChangeUnused; eauto. 
+    eauto. eauto. rewrite H5. rewrite UnionSubtract. unfoldTac. rewrite UnionSwap; eauto. }
   }
-Qed.
+Qed. 
 
 Theorem newSimActionStepsEmpty : forall H T H' T' TID x M' E d N N' H'' T'' N'' s2 s1 s1' a,
        eraseTrm (s1'++[a]) N' N'' ->
@@ -159,55 +160,56 @@ Proof.
    replace[a;nAct M' E d x0] with ([a]++[nAct M' E d x0]) in H6; auto. 
    rewrite app_assoc in H6. apply app_inj_tail in H6. invertHyp. rewrite H2 in H1. 
    inv H1. constructor. }
-  {startIndCase. eqIn H6. inv H7.   
-   {copy H9. apply pullOut in H9. rewrite H9. clear H9. copy H5. eapply specStepEmptyIVar' in H5; eauto. 
-    copy H5. eapply IHspec_multistep in H5;[idtac|eauto|idtac|auto|auto|auto|auto|auto]; auto.
-    takeTStep. eapply stepReplaceEmpty. auto. eapply H10. eapply specStepChangeUnused. 
-    eauto. unfoldTac. rewrite <- UnionSwap. eassumption. eapply spec_multi_trans. eassumption. 
-    takeTStep. repeat rewrite subtractSingle. constructor. proveUnionEq x.
-    rewrite subtractSingle. auto. }
-   {inv H9. apply UnionEqTID in x. invertHyp. inv H7. copy H5. eapply specStepEmptyIVar' in H5; eauto.  
-    inversion H7; subst; unfoldTac; invertHyp; invThreadEq.  
+  {startIndCase. destructThread x1. exMid H11 TID. 
+   {apply UnionEqTID in x. invertHyp. inv H7. copy H5. eapply specStepEmptyIVar' in H5; eauto.  
+    inversion H6; subst. 
     {copy H3. eapply stackNonNil in H3; eauto. destruct s1. exfalso. apply H3. auto. 
      econstructor. eapply SBasicStep; eauto. constructor. eapply IHspec_multistep; eauto. 
      eapply spec_multi_trans. eauto. econstructor. eapply SBasicStep; eauto. constructor.
-     intros c. subst. apply eraseTrmApp in H0. inv H0; inv H12; falseDecomp. }
+     intros c. subst. apply eraseTrmApp in H0. inv H0; inv H16; falseDecomp. }
     {econstructor. eapply SFork; eauto. simpl. unfoldTac. rewrite coupleUnion. 
-     rewrite <- Union_associative. rewrite UnionSwap. eapply IHspec_multistep; eauto. 
-     Focus 2. rewrite Union_associative. rewrite <- coupleUnion. rewrite couple_swap. 
+     rewrite Union_associative. rewrite UnionSwap. eapply IHspec_multistep; eauto. 
+     Focus 2. rewrite <- Union_associative. rewrite <- coupleUnion. rewrite couple_swap. 
      unfold numForks. simpl. simpl. eauto. rewrite numForksDistribute. simpl. rewrite <- plus_assoc. 
      rewrite <- plus_comm. simpl. rewrite plus_comm. reflexivity. eapply spec_multi_trans. 
-     eassumption. econstructor. eapply SFork; eauto. rewrite Union_associative. rewrite <- coupleUnion. 
+     eassumption. econstructor. eapply SFork; eauto. rewrite <- Union_associative. rewrite <- coupleUnion. 
      rewrite couple_swap. simpl. rewrite numForksDistribute. simpl. rewrite <- plus_assoc. 
      rewrite plus_comm. simpl. rewrite plus_comm. constructor. }
     {destruct(beq_nat x x0) eqn:eq. 
-     {apply beq_nat_true in eq. subst. rewrite H1 in H12. inv H12. }
+     {apply beq_nat_true in eq. subst. heapsDisagree. }
      {apply beq_nat_false in eq. apply neqSym in eq. lookupTac.
-      eapply IHspec_multistep in H10;[idtac|eauto|idtac|auto|auto|auto|auto|auto]; auto.
+      eapply IHspec_multistep in H7;[idtac|eauto|idtac|auto|auto|auto|auto|auto]; auto.
       econstructor. eapply SGet with(x:=x); auto. rewrite lookupReplaceNeq; eauto. 
       rewrite lookupReplaceSwitch; auto. eassumption. eapply spec_multi_trans. eassumption. 
       econstructor. eapply SGet with(x:=x); eauto. constructor. simpl. eauto. }
     }
-    {destruct (beq_nat x x0) eqn:eq. apply beq_nat_true in eq. subst. rewrite H12 in H1. 
+    {destruct (beq_nat x x0) eqn:eq. apply beq_nat_true in eq. subst. rewrite H16 in H1. 
      inv H1. eapply smultiEmptyFull in H4; eauto. contradiction. erewrite HeapLookupReplace; eauto. 
      apply beq_nat_false in eq. apply neqSym in eq. lookupTac.
-     eapply IHspec_multistep in H10;[idtac|eauto|idtac|auto|auto|auto|auto|auto]; auto.
+     eapply IHspec_multistep in H7;[idtac|eauto|idtac|auto|auto|auto|auto|auto]; auto.
      econstructor. eapply SPut with(x:=x). 
      rewrite lookupReplaceNeq; eauto. auto. rewrite lookupReplaceSwitch; auto. simpl. 
      eassumption. eapply spec_multi_trans. eassumption. econstructor. eapply SPut with(x:=x). 
      eauto. auto. constructor. simpl. reflexivity. }
-    {destruct (beq_nat x x0) eqn:eq. apply beq_nat_true in eq. subst. copy p. rewrite H10 in H1. 
+    {destruct (beq_nat x x0) eqn:eq. apply beq_nat_true in eq. subst. copy p. rewrite H7 in H1. 
      inv H1. apply beq_nat_false in eq. apply neqSym in eq. lookupTac.
-     eapply IHspec_multistep in H10;[idtac|eauto|idtac|auto|auto|auto|auto|auto]; auto.
+     eapply IHspec_multistep in H7;[idtac|eauto|idtac|auto|auto|auto|auto|auto]; auto.
      econstructor. eapply SNew with(x:=x). 
      auto. erewrite extendReplaceSwitch; eauto. eapply spec_multi_trans. eassumption. 
      econstructor. eapply SNew with(x:=x); eauto. constructor. simpl. auto. }
-    {econstructor. eapply SSpec; eauto. unfoldTac. rewrite coupleUnion. rewrite <- Union_associative. 
-     rewrite <- UnionSwap. eapply IHspec_multistep; eauto. Focus 2. rewrite Union_associative. 
+    {econstructor. eapply SSpec; eauto. unfoldTac. rewrite coupleUnion. rewrite Union_associative. 
+     rewrite <- UnionSwap. eapply IHspec_multistep; eauto. Focus 2. rewrite <- Union_associative. 
      rewrite <- coupleUnion.  rewrite couple_swap. reflexivity. eapply spec_multi_trans. 
-     eassumption. econstructor. eapply SSpec; eauto. rewrite Union_associative. rewrite <- coupleUnion. 
+     eassumption. econstructor. eapply SSpec; eauto. rewrite <- Union_associative. rewrite <- coupleUnion. 
      rewrite couple_swap. constructor. }
    }
+   {apply UnionNeqTID in x; auto. invertHyp.  copy H5. eapply specStepEmptyIVar' in H5; eauto. 
+    copy H5. eapply IHspec_multistep in H5;[idtac|eauto|idtac|auto|auto|auto|auto|auto]; auto.
+    rewrite H13. unfoldTac. rewrite UnionSwap. econstructor. eapply stepReplaceEmpty. eauto. 
+    eapply H15. eapply specStepChangeUnused; eauto. unfoldTac. rewrite UnionSwap; eauto. 
+    eapply spec_multi_trans. eassumption. rewrite H13. unfoldTac. rewrite UnionSwap. 
+    econstructor. eapply specStepChangeUnused; eauto. unfoldTac. rewrite UnionSwap. constructor. 
+    rewrite H6. rewrite UnionSubtract. unfoldTac. rewrite UnionSwap; eauto. }
   }
   Grab Existential Variables. rewrite lookupReplaceNeq; eauto. 
 Qed. 
@@ -222,7 +224,6 @@ Proof.
   {eauto. }
   {eapply specStepFullIVar in H; eauto. invertHyp. eauto. }
 Qed. 
-  
 
 Theorem specStepEmptyIVarOr : forall x H H' H'' T T' t t' s s' ds M t0,
                               heap_lookup x H = Some(sempty s) -> 
@@ -233,183 +234,33 @@ Theorem specStepEmptyIVarOr : forall x H H' H'' T T' t t' s s' ds M t0,
                                exists ds', heap_lookup x H' = Some(sfull s ds' s' t0 M)). 
 Proof. 
   intros. inversion H1; subst; eauto. 
-  {unfold tSingleton in *; invertHyp. destruct (beq_nat x x0)eqn:eq. 
+  {destruct (beq_nat x x0)eqn:eq. 
    {apply beq_nat_true in eq. subst. rewrite H5 in H0. inv H0. }
    {apply beq_nat_false in eq. rewrite lookupReplaceNeq; eauto. }
   }
-  {unfold tSingleton in *; invertHyp. destruct (beq_nat x x0)eqn:eq. 
+  {destruct (beq_nat x x0)eqn:eq. 
    {apply beq_nat_true in eq. subst. rewrite H5 in H0. inv H0.
     eapply smultiFullIVar in H2; eauto. Focus 2. erewrite HeapLookupReplace; eauto. 
     invertHyp. rewrite H3 in H0. inv H0. right. exists nil. erewrite HeapLookupReplace; eauto. }
    {apply beq_nat_false in eq. rewrite lookupReplaceNeq; eauto. }
   }
-  {unfold tSingleton in *; invertHyp. destruct (beq_nat x x0)eqn:eq. 
+  { destruct (beq_nat x x0)eqn:eq. 
    {apply beq_nat_true in eq. subst. copy p. rewrite H4 in H0. inv H0. }
    {apply beq_nat_false in eq. left. apply lookupExtendNeq; auto. }
   }
 Qed. 
 
-Theorem newSimPureStepsFull' : forall H T H' T' TID x M' E d M'' t0 ds ds' N N' N'' s2 s1',
-       eraseTrm s1' N' N'' -> 
-       heap_lookup x H = Some(sfull SPEC ds SPEC t0 M'') ->
-       heap_lookup x H' = Some(sfull SPEC ds' SPEC t0 M'')-> 
-       spec_multistep H (tUnion T (tSingleton(TID,unlocked[nAct M' E d x],s2,N))) H'
-                      (tUnion T' (tSingleton(TID,unlocked(s1'++[nAct M' E d x]),s2,N'))) ->
-       exists H'' T'',
-         spec_multistep H (tUnion T (tSingleton(TID,unlocked[nAct M' E d x],s2,N))) 
-                        H'' (tUnion T'' (tSingleton(TID,unlocked[nAct M' E d x],s2,N''))) /\
-         spec_multistep H'' (tUnion T'' (tSingleton(TID,unlocked[nAct M' E d x],s2,N''))) 
-                        H' (tUnion T' (tSingleton(TID,unlocked(s1'++[nAct M' E d x]),s2,N'))) /\
-         exists ds'',
-         spec_multistep (replace x (sfull COMMIT ds SPEC t0 M'') H) T 
-                        (replace x (sfull COMMIT ds'' SPEC t0 M'')H'') T'' /\
-          heap_lookup x H'' = Some(sfull SPEC ds'' SPEC t0 M''). 
-Proof.
-  intros. genDeps{ds; ds'}. dependent induction H3; intros. 
-  {apply UnionEqTID in x. invertHyp. inv H. destruct s1'; inv H5; try invertListNeq. 
-   inv H0; try invertListNeq. rewrite H1 in H2. inv H2. do 6 econstructor. constructor. 
-   eauto. }
-  {startIndCase. eqIn H5. inv H6. 
-   {copy H4. destruct x1. destruct p. destruct p. copy H1. eapply specStepFullIVar' in H1; eauto. inv H1. 
-    {copy H10. eapply IHspec_multistep in H10; eauto. Focus 2. proveUnionEq x. invertHyp. 
-     econstructor. econstructor. split. takeTStep. eauto. split; eauto. econstructor. 
-     split. Focus 2. eauto. apply pullOut in H8. rewrite H8. clear H8. 
-     inversion H9; unfoldTac; invertHyp; invThreadEq. 
-     {econstructor. eapply SBasicStep; eauto. eauto. }
-     {econstructor. eapply SFork; eauto. eauto. }
-     {varsEq x4 x0. rewrite H12 in H4. inv H4. erewrite HeapLookupReplace in H1; eauto. 
-      inversion H1. invertListNeq. econstructor. eapply SGet; eauto.
-      rewrite lookupReplaceNeq; eauto. rewrite lookupReplaceSwitch; eauto. }
-     {varsEq x4 x0. heapsDisagree. econstructor. eapply SPut; eauto. 
-      rewrite lookupReplaceNeq; eauto. rewrite lookupReplaceSwitch; eauto. }
-     {varsEq x4 x0. copy p. heapsDisagree. econstructor. eapply SNew; eauto. 
-      erewrite extendReplaceSwitch; eauto. }
-     {econstructor. eapply SSpec; eauto. eauto. }
-    }
-    {inversion H9; unfoldTac; invertHyp; invThreadEq. 
-     {rewrite H10 in H4. inversion H4. invertListNeq. }
-     {rewrite H10 in H4. inversion H4; invertListNeq. }
-     {varsEq x1 x0. 
-      {lookupTac. rewrite H11 in H4. inv H4. eapply IHspec_multistep in H1; eauto. 
-       Focus 2. proveUnionEq x. invertHyp. econstructor. econstructor. split. 
-       takeTStep. eauto. split; eauto. econstructor. split. apply pullOut in H8. 
-       rewrite H8. econstructor. eapply SGet; eauto. erewrite HeapLookupReplace; eauto.
-       rewrite replaceOverwrite. rewrite replaceOverwrite in H13. eauto. eauto. }
-      {rewrite lookupReplaceNeq in H10; eauto. rewrite H10 in H4. inversion H4. invertListNeq. }
-     }
-     {varsEq x1 x0. heapsDisagree. rewrite lookupReplaceNeq in H10. rewrite H10 in H4. 
-      inversion H4; invertListNeq. auto. }
-     {varsEq x1 x0. heapsDisagree. erewrite lookupExtendNeq in H10; eauto. inversion H10. 
-      invertListNeq. }
-     {rewrite H10 in H4. inversion H4; invertListNeq. }
-    }
-   }
-   {inv H8. apply UnionEqTID in x. invertHyp. inversion H1; unfoldTac; invertHyp; invThreadEq. 
-    {eapply IHspec_multistep in H4;[idtac|eauto|idtac|eauto|eauto|eauto|eauto]. Focus 2. auto.
-     invertHyp. econstructor. econstructor. split. econstructor. eapply SBasicStep; eauto. 
-     eauto. split; auto. econstructor. split. eauto. eauto. }
-    {copy H3. nonEmptyStackTac H3. invertHyp. apply eraseTrmApp in H0. inv H0. do 4 econstructor. 
-     econstructor. eapply SFork; eauto. eassumption. econstructor. split. constructor. eauto. }
-    {copy H3. nonEmptyStackTac H3. invertHyp. apply eraseTrmApp in H0. inv H0. do 4 econstructor. 
-     econstructor. eapply SGet; eauto. eassumption. econstructor. split. constructor. eauto. }
-    {copy H3. nonEmptyStackTac H3. invertHyp. apply eraseTrmApp in H0. inv H0. do 4 econstructor. 
-     econstructor. eapply SPut; eauto. eassumption. econstructor. split. constructor. eauto. }
-    {copy H3. nonEmptyStackTac H3. invertHyp. apply eraseTrmApp in H0. inv H0. do 4 econstructor. 
-     econstructor. eapply SNew; eauto. eassumption. econstructor. split. constructor. eauto. }
-    {copy H3. nonEmptyStackTac H3. invertHyp. apply eraseTrmApp in H0. inv H0. do 4 econstructor. 
-     econstructor. eapply SSpec; eauto. eassumption. econstructor. split. constructor. eauto. }
-   }
-  }
-  Grab Existential Variables. rewrite lookupReplaceNeq; eauto. 
-Qed. 
-
-Theorem newSimPureStepsFull : forall H T H' T' TID x M' E d M'' t0 ds' N N' N'' s2 s1',
-       eraseTrm s1' N' N'' -> 
-       heap_lookup x H = Some(sempty SPEC) ->
-       heap_lookup x H' = Some(sfull SPEC ds' SPEC t0 M'')-> 
-       spec_multistep H (tUnion T (tSingleton(TID,unlocked[nAct M' E d x],s2,N))) H'
-                      (tUnion T' (tSingleton(TID,unlocked(s1'++[nAct M' E d x]),s2,N'))) ->
-       (exists H'' T'',
-         spec_multistep H (tUnion T (tSingleton(TID,unlocked[nAct M' E d x],s2,N))) 
-                        H'' (tUnion T'' (tSingleton(TID,unlocked[nAct M' E d x],s2,N''))) /\
-         spec_multistep H'' (tUnion T'' (tSingleton(TID,unlocked[nAct M' E d x],s2,N''))) 
-                        H' (tUnion T' (tSingleton(TID,unlocked(s1'++[nAct M' E d x]),s2,N'))) /\
-         spec_multistep (replace x (sempty COMMIT) H) T 
-                        (replace x (sempty COMMIT)H'') T'' /\
-          heap_lookup x H'' = Some(sempty SPEC)) \/
-       (exists H'' T'' ds'',
-         spec_multistep H (tUnion T (tSingleton(TID,unlocked[nAct M' E d x],s2,N))) 
-                        H'' (tUnion T'' (tSingleton(TID,unlocked[nAct M' E d x],s2,N''))) /\
-         spec_multistep H'' (tUnion T'' (tSingleton(TID,unlocked[nAct M' E d x],s2,N''))) 
-                        H' (tUnion T' (tSingleton(TID,unlocked(s1'++[nAct M' E d x]),s2,N'))) /\
-         spec_multistep (replace x (sempty COMMIT) H) T 
-                        (replace x (sfull COMMIT ds'' SPEC t0 M'')H'') T'' /\
-          heap_lookup x H'' = Some(sfull SPEC ds'' SPEC t0 M'')). 
-Proof.
-  intros. dependent induction H3. 
-  {rewrite H1 in H2. inv H2. }
-  {startIndCase. eqIn H5. inv H6. 
-   {copy H4. eapply specStepEmptyIVarOr in H4; eauto. inv H4. 
-    {copy H9. eapply IHspec_multistep in H9; eauto. Focus 2. proveUnionEq x. inv H9. 
-     {invertHyp. left. econstructor. econstructor. split. takeTStep. eassumption. 
-      split. assumption. split. apply pullOut in H8. rewrite H8. econstructor. 
-      eapply stepReplaceEmpty. assumption. eapply H4. eapply specStepChangeUnused. 
-      eassumption. eauto. eauto. }
-     {invertHyp. right. econstructor. econstructor. econstructor. split. takeTStep. eauto. 
-      split; eauto. split. Focus 2. eauto. apply pullOut in H8. rewrite H8. clear H8. 
-      inversion H6; subst; unfoldTac; invertHyp. 
-      {econstructor. eapply SBasicStep; eauto. auto. }
-      {econstructor. eapply SFork; eauto. eauto. }
-      {varsEq x5 x0. heapsDisagree. econstructor. eapply SGet; eauto. 
-       rewrite lookupReplaceNeq; eauto. rewrite lookupReplaceSwitch; eauto. }
-      {varsEq x5 x0. erewrite HeapLookupReplace in H4; eauto. inv H4. econstructor. 
-       eapply SPut; eauto. rewrite lookupReplaceNeq; eauto. rewrite lookupReplaceSwitch; eauto. }
-      {varsEq x5 x0. heapsDisagree. econstructor. eapply SNew; eauto.
-       erewrite extendReplaceSwitch; eauto. }
-      {econstructor. eapply SSpec; eauto. eauto. }
-     }
-    }
-    {invertHyp. apply UnionSingletonEq in x; auto. rewrite x in H3. unfoldTac. rewrite UnionSwap in H3. 
-     eapply newSimPureStepsFull' in H3; eauto. invertHyp. right. econstructor. econstructor. econstructor. 
-     split. takeTStep. eauto. split; eauto. split.
-     inversion H6; unfoldTac; invertHyp; try solve[heapsDisagree]. 
-     {varsEq x5 x0. heapsDisagree. erewrite lookupReplaceNeq in H4; eauto. heapsDisagree. }
-     {varsEq x5 x0. erewrite HeapLookupReplace in H4; eauto. inv H4. apply pullOut in H8. 
-      rewrite H8. econstructor. eapply SPut; eauto. erewrite HeapLookupReplace; eauto. 
-      rewrite replaceOverwrite. rewrite replaceOverwrite in H11. eauto. 
-      rewrite lookupReplaceNeq in H4; eauto. heapsDisagree. }
-     {varsEq x5 x0. heapsDisagree. erewrite lookupExtendNeq in H4; eauto. inv H4. }
-     eauto. 
-    }
-   }
-   {inv H8. apply UnionEqTID in x. invertHyp. inversion H4; unfoldTac; invertHyp; invThreadEq. 
-    {eapply IHspec_multistep in H1;[idtac|eauto|idtac|auto|auto|auto|auto]. Focus 2. auto. 
-     inv H1. 
-     {invertHyp. left. econstructor. econstructor. split. econstructor. eapply SBasicStep; eauto. 
-      eassumption. split; auto. }
-     {right. invertHyp. econstructor. econstructor. econstructor. split. econstructor.
-      eapply SBasicStep; eauto. eauto. eauto. }
-    }
-    {copy H3. nonEmptyStackTac H3. invertHyp. apply eraseTrmApp in H0. inv H0. do 4 econstructor. 
-     constructor. split. simpl in *. econstructor. eapply SFork; eauto. eassumption. 
-     split. constructor. eauto. }
-    {copy H3. nonEmptyStackTac H3. invertHyp. apply eraseTrmApp in H0. inv H0. do 4 econstructor. 
-     constructor. split. simpl in *. econstructor. eapply SGet; eauto. eassumption. 
-     split. constructor. eauto. }
-    {copy H3. nonEmptyStackTac H3. invertHyp. apply eraseTrmApp in H0. inv H0. do 4 econstructor. 
-     constructor. split. simpl in *. econstructor. eapply SPut; eauto. eassumption. 
-     split. constructor. eauto. }
-    {copy H3. nonEmptyStackTac H3. invertHyp. apply eraseTrmApp in H0. inv H0. do 4 econstructor. 
-     constructor. split. simpl in *. econstructor. eapply SNew; eauto. eassumption. 
-     split. constructor. eauto. }
-    {copy H3. nonEmptyStackTac H3. invertHyp. apply eraseTrmApp in H0. inv H0. do 4 econstructor. 
-     constructor. split. simpl in *. econstructor. eapply SSpec; eauto. eassumption. 
-     split. constructor. eauto. }
-   }
-  }
-  Grab Existential Variables. rewrite lookupReplaceNeq; eauto. 
-Qed. 
-
+Ltac takeTStep :=
+  match goal with
+      |H:?T = ?x |- _ =>
+       rewrite H; unfoldTac; rewrite UnionSwap; 
+       econstructor;[eapply specStepChangeUnused; eassumption|idtac]; unfoldTac; 
+       rewrite <- UnionSwap                                          
+      |H:?T = ?x |- _ =>
+       rewrite H; unfoldTac; rewrite UnionSwap
+      |H:?T = ?x |- _ =>
+       rewrite H
+  end. 
 
 Theorem stepReplaceSpecFull : forall H T H' t t' ds ds' x M' TID,
                    heap_lookup x H = Some(sfull SPEC ds SPEC TID M') ->
@@ -447,6 +298,146 @@ Proof.
    eapply stepReplaceSpecFull in H3; eauto. econstructor. eassumption.
    eapply IHspec_multistep; eauto. }
 Qed. 
+
+Theorem newSimPureStepsFull' : forall H T H' T' TID x M' E d M'' t0 ds ds' N N' N'' s2 s1',
+       eraseTrm s1' N' N'' -> 
+       heap_lookup x H = Some(sfull SPEC ds SPEC t0 M'') ->
+       heap_lookup x H' = Some(sfull SPEC ds' SPEC t0 M'')-> 
+       spec_multistep H (tUnion T (tSingleton(TID,unlocked[nAct M' E d x],s2,N))) H'
+                      (tUnion T' (tSingleton(TID,unlocked(s1'++[nAct M' E d x]),s2,N'))) ->
+       exists H'' T'',
+         spec_multistep H (tUnion T (tSingleton(TID,unlocked[nAct M' E d x],s2,N))) 
+                        H'' (tUnion T'' (tSingleton(TID,unlocked[nAct M' E d x],s2,N''))) /\
+         spec_multistep H'' (tUnion T'' (tSingleton(TID,unlocked[nAct M' E d x],s2,N''))) 
+                        H' (tUnion T' (tSingleton(TID,unlocked(s1'++[nAct M' E d x]),s2,N'))) /\
+         exists ds'',
+         spec_multistep (replace x (sfull COMMIT ds SPEC t0 M'') H) T 
+                        (replace x (sfull COMMIT ds'' SPEC t0 M'')H'') T'' /\
+          heap_lookup x H'' = Some(sfull SPEC ds'' SPEC t0 M''). 
+Proof.
+  intros. genDeps{ds; ds'}. dependent induction H3; intros. 
+  {apply UnionEqTID in x. invertHyp. inv H. destruct s1'; inv H5; try invertListNeq. 
+   inv H0; try invertListNeq. rewrite H1 in H2. inv H2. do 6 econstructor. constructor. 
+   eauto. }
+  {startIndCase. destructThread x1. exMid TID H10. 
+   {apply UnionEqTID in x. invertHyp. inversion H1; subst. 
+    {eapply IHspec_multistep in H4;[idtac|eauto|idtac|eauto|eauto|eauto|eauto]. Focus 2. auto.
+     invertHyp. econstructor. econstructor. split. econstructor. eapply SBasicStep; eauto. 
+     eauto. split; auto. econstructor. split. eauto. eauto. }
+    {copy H3. nonEmptyStackTac H3. invertHyp. apply eraseTrmApp in H0. inv H0. do 4 econstructor. 
+     econstructor. eapply SFork; eauto. eassumption. econstructor. split. constructor. eauto. }
+    {copy H3. nonEmptyStackTac H3. invertHyp. apply eraseTrmApp in H0. inv H0. do 4 econstructor. 
+     econstructor. eapply SGet; eauto. eassumption. econstructor. split. constructor. eauto. }
+    {copy H3. nonEmptyStackTac H3. invertHyp. apply eraseTrmApp in H0. inv H0. do 4 econstructor. 
+     econstructor. eapply SPut; eauto. eassumption. econstructor. split. constructor. eauto. }
+    {copy H3. nonEmptyStackTac H3. invertHyp. apply eraseTrmApp in H0. inv H0. do 4 econstructor. 
+     econstructor. eapply SNew; eauto. eassumption. econstructor. split. constructor. eauto. }
+    {copy H3. nonEmptyStackTac H3. invertHyp. apply eraseTrmApp in H0. inv H0. do 4 econstructor. 
+     econstructor. eapply SSpec; eauto. eassumption. econstructor. split. constructor. eauto. }
+   }
+   {copy H4. copy H1. eapply specStepFullIVar in H1; eauto. invertHyp.  
+    apply UnionNeqTID in x. invertHyp. copy H13. eapply IHspec_multistep in H13; eauto. 
+    invertHyp. econstructor. econstructor. split. takeTStep. eauto. split; auto. 
+    econstructor. split. Focus 2. eauto. rewrite H14. econstructor.
+    eapply stepReplaceSpecFull. eauto. eapply H15. eapply specStepChangeUnused; eauto. 
+    eauto. rewrite H1. rewrite UnionSubtract. unfoldTac; rewrite UnionSwap; eauto. auto. }
+  }
+Qed. 
+
+Theorem newSimPureStepsFull : forall H T H' T' TID x M' E d M'' t0 ds' N N' N'' s2 s1',
+       eraseTrm s1' N' N'' -> 
+       heap_lookup x H = Some(sempty SPEC) ->
+       heap_lookup x H' = Some(sfull SPEC ds' SPEC t0 M'')-> 
+       spec_multistep H (tUnion T (tSingleton(TID,unlocked[nAct M' E d x],s2,N))) H'
+                      (tUnion T' (tSingleton(TID,unlocked(s1'++[nAct M' E d x]),s2,N'))) ->
+       (exists H'' T'',
+         spec_multistep H (tUnion T (tSingleton(TID,unlocked[nAct M' E d x],s2,N))) 
+                        H'' (tUnion T'' (tSingleton(TID,unlocked[nAct M' E d x],s2,N''))) /\
+         spec_multistep H'' (tUnion T'' (tSingleton(TID,unlocked[nAct M' E d x],s2,N''))) 
+                        H' (tUnion T' (tSingleton(TID,unlocked(s1'++[nAct M' E d x]),s2,N'))) /\
+         spec_multistep (replace x (sempty COMMIT) H) T 
+                        (replace x (sempty COMMIT)H'') T'' /\
+          heap_lookup x H'' = Some(sempty SPEC)) \/
+       (exists H'' T'' ds'',
+         spec_multistep H (tUnion T (tSingleton(TID,unlocked[nAct M' E d x],s2,N))) 
+                        H'' (tUnion T'' (tSingleton(TID,unlocked[nAct M' E d x],s2,N''))) /\
+         spec_multistep H'' (tUnion T'' (tSingleton(TID,unlocked[nAct M' E d x],s2,N''))) 
+                        H' (tUnion T' (tSingleton(TID,unlocked(s1'++[nAct M' E d x]),s2,N'))) /\
+         spec_multistep (replace x (sempty COMMIT) H) T 
+                        (replace x (sfull COMMIT ds'' SPEC t0 M'')H'') T'' /\
+          heap_lookup x H'' = Some(sfull SPEC ds'' SPEC t0 M'')). 
+Proof.
+  intros. dependent induction H3. 
+  {rewrite H1 in H2. inv H2. }
+  {startIndCase. destructThread x1. exMid H10 TID. 
+   {apply UnionEqTID in x. invertHyp. inversion H4; subst.
+    {eapply IHspec_multistep in H1;[idtac|eauto|idtac|auto|auto|auto|auto]. Focus 2. auto. 
+     inv H1. 
+     {invertHyp. left. econstructor. econstructor. split. econstructor. eapply SBasicStep; eauto. 
+      eassumption. split; auto. }
+     {right. invertHyp. econstructor. econstructor. econstructor. split. econstructor.
+      eapply SBasicStep; eauto. eauto. eauto. }
+    }
+    {copy H3. nonEmptyStackTac H3. invertHyp. apply eraseTrmApp in H0. inv H0. do 4 econstructor. 
+     constructor. split. simpl in *. econstructor. eapply SFork; eauto. eassumption. 
+     split. constructor. eauto. }
+    {copy H3. nonEmptyStackTac H3. invertHyp. apply eraseTrmApp in H0. inv H0. do 4 econstructor. 
+     constructor. split. simpl in *. econstructor. eapply SGet; eauto. eassumption. 
+     split. constructor. eauto. }
+    {copy H3. nonEmptyStackTac H3. invertHyp. apply eraseTrmApp in H0. inv H0. do 4 econstructor. 
+     constructor. split. simpl in *. econstructor. eapply SPut; eauto. eassumption. 
+     split. constructor. eauto. }
+    {copy H3. nonEmptyStackTac H3. invertHyp. apply eraseTrmApp in H0. inv H0. do 4 econstructor. 
+     constructor. split. simpl in *. econstructor. eapply SNew; eauto. eassumption. 
+     split. constructor. eauto. }
+    {copy H3. nonEmptyStackTac H3. invertHyp. apply eraseTrmApp in H0. inv H0. do 4 econstructor. 
+     constructor. split. simpl in *. econstructor. eapply SSpec; eauto. eassumption. 
+     split. constructor. eauto. }
+   }
+   {copy H4. eapply specStepEmptyIVarOr in H4; eauto. inv H4. 
+    {copy H12. eapply IHspec_multistep in H12; eauto. inv H12. 
+     {apply UnionNeqTID in x. invertHyp. left. econstructor. econstructor. 
+      split. takeTStep. eassumption. split. assumption. split. rewrite H17. econstructor. 
+      eapply stepReplaceEmpty. auto. eapply H4. eapply specStepChangeUnused. eauto.
+      eauto. eauto. eauto. }
+     {apply UnionNeqTID in x; auto. invertHyp. right. econstructor. econstructor. econstructor. 
+      split. takeTStep. eauto. split; eauto. split. Focus 2. eauto. rewrite H17. clear H15 H17.
+      inversion H5; subst.
+      {econstructor. eapply SBasicStep; eauto. auto. }
+      {econstructor. eapply SFork; eauto. eauto. }
+      {varsEq x x0. heapsDisagree. econstructor. eapply SGet; eauto. 
+       rewrite lookupReplaceNeq; eauto. rewrite lookupReplaceSwitch; eauto. }
+      {varsEq x x0. erewrite HeapLookupReplace in H4; eauto. inv H4. econstructor. 
+       eapply SPut; eauto. rewrite lookupReplaceNeq; eauto. rewrite lookupReplaceSwitch; eauto. }
+      {varsEq x x0. heapsDisagree. econstructor. eapply SNew; eauto.
+       erewrite extendReplaceSwitch; eauto. }
+      {econstructor. eapply SSpec; eauto. eauto. }
+     }
+     {proveUnionEq x. rewrite UnionSubtract. rewrite UnionSwap; auto. 
+      apply UnionNeqTID in x. invertHyp. rewrite H14. solveSet. auto. }
+    }
+    {invertHyp. apply UnionNeqTID in x. invertHyp. rewrite H12 in H3. unfoldTac. 
+     rewrite UnionSwap in H3. eapply newSimPureStepsFull' in H3. invertHyp. 
+     right. econstructor. econstructor. econstructor. split. takeTStep. eauto. split; eauto. split.
+     inversion H6; unfoldTac; invertHyp; try solve[heapsDisagree]. 
+     {varsEq x5 x0. heapsDisagree. erewrite lookupReplaceNeq in H4; eauto. heapsDisagree. }
+     {varsEq x5 x0. erewrite HeapLookupReplace in H4; eauto. inv H4. apply pullOut in H8. 
+      rewrite H8. econstructor. eapply SPut; eauto. erewrite HeapLookupReplace; eauto. 
+      rewrite replaceOverwrite. rewrite replaceOverwrite in H11. eauto. 
+      rewrite lookupReplaceNeq in H4; eauto. heapsDisagree. }
+     {varsEq x5 x0. heapsDisagree. erewrite lookupExtendNeq in H4; eauto. inv H4. }
+     eauto. 
+    }
+   }
+
+
+
+
+  Grab Existential Variables. rewrite lookupReplaceNeq; eauto. 
+Qed. 
+
+
+
 
 Theorem smultiReplaceEmptyFull : forall H T H' T' ds' x M' TID,
                    heap_lookup x H = Some(sempty SPEC) ->
