multiset/writeIndependence.v
@@ -1,155 +1,17 @@
 Require Import erasure. 
 Require Import IndependenceCommon. 
 
-Theorem writeFastForward : forall H T H' T' TID x M' E M'' s2 d s1' M,
-         heap_lookup x H = Some(sempty COMMIT) -> decompose M' E (put (fvar x) M'') ->
-         spec_multistep H (tUnion T (tSingleton(TID,unlocked nil,s2,M'))) H' 
-                        (tUnion T' (tSingleton(TID,unlocked(s1'++[wAct x M' E M'' d]),s2,M))) ->
-         exists H'' T'' ,
-           spec_multistep H (tUnion T (tSingleton(TID,unlocked nil,s2,M'))) H''
-                         (tUnion T'' (tSingleton(TID,unlocked [wAct x M' E M'' d],s2,fill E (ret unit)))) /\
-           spec_multistep H'' (tUnion T'' (tSingleton(TID,unlocked [wAct x M' E M'' d],s2,fill E (ret unit))))
-                          H' (tUnion T' (tSingleton(TID,unlocked(s1'++[wAct x M' E M'' d]),s2,M)))  /\
-           spec_multistep (replace x (sfull COMMIT nil COMMIT TID M'') H) T 
-                          (replace x (sfull COMMIT nil COMMIT TID M'')H'') T'' /\ 
-           heap_lookup x H'' = Some(sfull COMMIT nil SPEC TID M'').
-Proof.
-  intros. dependent induction H2. 
-  {apply UnionEqTID in x. invertHyp. inv H2. invertListNeq. }
-  {copy x. copy H3. apply specStepSingleton in H5. invertHyp. copy x. unfoldSetEq x.
-   assert(tIn (tUnion T0 (tSingleton x1)) x1). apply Union_intror. constructor.
-   apply H6 in H8. inv H8. 
-   {copy H3. eapply specStepEmptyIVar in H3; eauto. Focus 3. apply Union_intror. constructor.
-    eapply IHspec_multistep in H1. Focus 2. eassumption. Focus 2. auto. Focus 3. auto. 
-    invertHyp. exists x. exists x2.  split. copy H9. apply pullOut in H12. rewrite H12. 
-    unfoldTac. rewrite UnionSwap. econstructor. eapply specStepChangeUnused. eauto. 
-    unfoldTac. rewrite <- UnionSwap. eassumption. split. eassumption. split.
-    apply pullOut in H9. rewrite H9. clear H9. inv H8; unfoldTac; invertHyp.
-    {econstructor. eapply SBasicStep; eauto. auto. }
-    {econstructor. eapply SFork. auto. eauto. }
-    {destruct (beq_nat x3 x0) eqn:eq. apply beq_nat_true in eq. subst. 
-     erewrite HeapLookupReplace in H3; eauto. inv H3. econstructor. eapply SGet with(x:=x3). 
-     apply beq_nat_false in eq. rewrite lookupReplaceNeq; eauto. auto.  
-     rewrite lookupReplaceSwitch. unfoldTac. eassumption. apply beq_nat_false in eq. auto. }
-    {destruct (beq_nat x3 x0) eqn:eq. apply beq_nat_true in eq. subst.
-     erewrite HeapLookupReplace in H3; eauto. inv H3. econstructor. eapply SPut with(x:=x3). 
-     apply beq_nat_false in eq. rewrite lookupReplaceNeq; eauto. auto. 
-     rewrite lookupReplaceSwitch. eassumption. apply beq_nat_false in eq. auto. }
-    {destruct (beq_nat x3 x0)eqn:eq. apply beq_nat_true in eq. subst. rewrite lookupExtend in H3. 
-     inv H3. econstructor. eapply SNew with(x:=x3). auto. 
-     erewrite extendReplaceSwitch; eauto. apply beq_nat_false in eq. auto. }
-    {econstructor. eapply SSpec; eauto. eassumption. }
-    auto. apply UnionSingletonEq in H4. rewrite H4. unfoldTac. rewrite UnionSwap. auto. auto. 
-    apply UnionSingletonEq in H4. rewrite H4. constructor. apply Union_intror. constructor. auto. 
-   }
-   {inv H9. apply UnionEqTID in H4. invertHyp. clear H4 H9 H10. 
-    exists (replace x0 (sfull COMMIT nil SPEC TID M'') H). 
-    exists T. split. econstructor. 
-    eapply SPut. eauto. auto. simpl. constructor. split. inv H3; unfoldTac; invertHyp; invThreadEq. 
-    {inv H8; copy d; eapply uniqueCtxtDecomp in H; eauto; invertHyp; inv H8. }
-    {copy d. copy d0. eapply uniqueCtxtDecomp in H; eauto. invertHyp. inv H8. }
-    {copy d. copy d0. eapply uniqueCtxtDecomp in H3; eauto. invertHyp. solveByInv. }
-    {copy d. copy d0. eapply uniqueCtxtDecomp in H3; eauto. invertHyp. inv H10. copy H2. 
-     rewrite H0 in H8. inv H8. assert(d=d0). apply proof_irrelevance. subst. eassumption. }
-    {copy d; copy d0. eapply uniqueCtxtDecomp in H3; eauto. invertHyp.  solveByInv. }
-    {copy d; copy d0. eapply uniqueCtxtDecomp in H; eauto. invertHyp. solveByInv. }
-    split. rewrite replaceOverwrite. constructor. erewrite HeapLookupReplace; eauto. }
-  }
-  Grab Existential Variables. apply beq_nat_false in eq. rewrite lookupReplaceNeq; eauto. 
-Qed. 
-
-Theorem writeSimPureSteps : forall H T H' T' TID x M' E M'' d N N' N'' s2 s1' ds ds',
-       eraseTrm s1' N' N'' -> 
-       heap_lookup x H = Some(sfull COMMIT ds SPEC TID M'') ->       
-       heap_lookup x H' = Some(sfull COMMIT ds' SPEC TID M'') -> 
-       spec_multistep H (tUnion T (tSingleton(TID,unlocked[wAct x M' E M'' d],s2,N))) H'
-                      (tUnion T' (tSingleton(TID,unlocked(s1'++[wAct x M' E M'' d]),s2,N'))) ->
-       exists H'' T'',
-         spec_multistep H (tUnion T (tSingleton(TID,unlocked[wAct x M' E M'' d],s2,N))) 
-                        H'' (tUnion T'' (tSingleton(TID,unlocked[wAct x M' E M'' d],s2,N''))) /\
-         spec_multistep H'' (tUnion T'' (tSingleton(TID,unlocked[wAct x M' E M'' d],s2,N''))) 
-                        H' (tUnion T' (tSingleton(TID,unlocked(s1'++[wAct x M' E M'' d]),s2,N'))) /\
-         exists ds'',
-         spec_multistep (replace x (sfull COMMIT ds COMMIT TID M'') H) T 
-                        (replace x (sfull COMMIT ds'' COMMIT TID M'')H'') T'' /\
-         heap_lookup x H'' = Some(sfull COMMIT ds'' SPEC TID M'').
-Proof.
-  intros. genDeps{N'';ds; ds'}. dependent induction H3; intros.
-  {apply UnionEqTID in x. invertHyp. inv H. destruct s1'; inv H5. inv H0; try invertListNeq. 
-   rewrite H2 in H1. inv H1. repeat econstructor. eauto. invertListNeq. }
-   {copy x. copy H0. apply specStepSingleton in H6. invertHyp. unfoldSetEq H5. 
-   assert(tIn (tUnion T0(tSingleton x1)) x1). apply Union_intror. constructor. apply H6 in H5. 
-   inv H5.  
-   {copy H8. apply pullOut in H8. rewrite H8. clear H8. 
-    inversion H0; subst; unfoldTac; invertHyp. 
-    {eapply IHspec_multistep in H1;[idtac|eauto|eauto|eauto|eauto|eauto|eauto]. Focus 2.
-     proveUnionEq x. invertHyp. exists x1. exists x2. split. rewrite UnionSwap. econstructor. 
-     eapply specStepChangeUnused. eassumption. unfoldTac. rewrite <- UnionSwap. eassumption. 
-     split. eassumption. exists x3. split. econstructor. eapply SBasicStep; eauto. eassumption. 
-     eauto. }
-    {eapply IHspec_multistep in H1;[idtac|eauto|eauto|eauto|eauto|eauto|eauto]. Focus 2.
-     proveUnionEq x. invertHyp. exists x1. exists x2. split. rewrite UnionSwap. econstructor. 
-     eapply specStepChangeUnused. eassumption. unfoldTac. rewrite <- UnionSwap. eassumption. 
-     split. eassumption. exists x3. split. econstructor. eapply SFork; eauto. eassumption. 
-     eauto. }
-    {destruct (beq_nat x2 x0) eqn:eq. 
-     {apply beq_nat_true in eq. subst. rewrite H9 in H1. inv H1. lookupTac.
-      eapply IHspec_multistep in H1; eauto. Focus 2. proveUnionEq x.  
-      invertHyp. exists x1. exists x2. split. rewrite UnionSwap. econstructor. eapply SGet. 
-      eauto. auto. unfoldTac. rewrite <- UnionSwap. eassumption. split. eauto. exists x3. split. 
-      econstructor. eapply SGet with (x:=x0). erewrite HeapLookupReplace; eauto. auto. 
-      rewrite replaceOverwrite. rewrite replaceOverwrite in H11. eapply H11. eassumption. }
-     {apply beq_nat_false in eq. rewrite neqSym in eq. lookupTac. eapply IHspec_multistep in H8; eauto. 
-      Focus 2. proveUnionEq x. invertHyp. exists x1. exists x3. split. rewrite UnionSwap. econstructor.
-      eapply SGet with(x:=x2). eassumption. auto. unfoldTac. rewrite <- UnionSwap. eassumption. 
-      split. eassumption. exists x4. split. econstructor. eapply SGet with(x:=x2). 
-      rewrite lookupReplaceNeq. eauto. auto. auto. rewrite lookupReplaceSwitch. eassumption. 
-      auto. eauto. }
-    }
-    {destruct (beq_nat x2 x0) eqn:eq. apply beq_nat_true in eq. subst. rewrite H9 in H1. 
-     inv H1. apply beq_nat_false in eq. rewrite neqSym in eq. lookupTac.
-     eapply IHspec_multistep in H8; eauto. Focus 2. proveUnionEq x. invertHyp. exists x1. 
-     exists x3. split. rewrite UnionSwap. econstructor. eapply SPut; eauto. unfoldTac. 
-     rewrite <- UnionSwap. eassumption. split. eassumption. exists x4. split. econstructor. 
-     eapply SPut with(x:=x2); eauto. rewrite lookupReplaceNeq. eauto. auto. 
-     rewrite lookupReplaceSwitch; auto. eassumption. eauto. }
-    {destruct (beq_nat x2 x0) eqn:eq. apply beq_nat_true in eq. subst. copy p. rewrite H8 in H1. 
-     inv H1. apply beq_nat_false in eq. rewrite neqSym in eq. lookupTac. 
-     eapply IHspec_multistep in H8; eauto. Focus 2. proveUnionEq x. invertHyp. exists x1. 
-     exists x3. split. rewrite UnionSwap. econstructor. eapply SNew; eauto. unfoldTac. 
-     rewrite <- UnionSwap. eassumption. split. eassumption. exists x4. split. econstructor. 
-     eapply SNew with(x:=x2); eauto. erewrite extendReplaceSwitch; eauto. eauto. 
-    }
-    {eapply IHspec_multistep in H1;[idtac|eauto|eauto|eauto|eauto|eauto|eauto]. Focus 2.
-     proveUnionEq x. invertHyp. exists x1. exists x2. split. rewrite UnionSwap. econstructor. 
-     eapply specStepChangeUnused. eassumption. unfoldTac. rewrite <- UnionSwap. eassumption. 
-     split. eassumption. exists x3. split. econstructor. eapply SSpec. eauto. eauto. 
-    }
-   }
-   {inv H8. apply UnionEqTID in x. invertHyp. inv H0; unfoldTac; invertHyp; invThreadEq. 
-    {eapply IHspec_multistep in H1;[idtac|eauto|eauto|eauto|eauto|eauto|eauto]. invertHyp. 
-     exists x. exists x1. split. econstructor. eapply SBasicStep; eauto. eassumption. 
-     split. eassumption. exists x2. split. assumption. eassumption. }
-    {copy H3. nonEmptyStackTac H3. invertHyp. apply eraseTrmApp in H4. inv H4. exists h'. 
-     exists T. split. constructor. split. simpl in *. econstructor. eapply SFork; eauto. 
-     eassumption. econstructor. split. constructor. eauto. }
-    {copy H3. nonEmptyStackTac H3. invertHyp. apply eraseTrmApp in H4. inv H4. 
-     exists H. exists T. split. constructor. split. simpl in *. econstructor. 
-     eapply SGet; eauto. eassumption. econstructor. split. constructor. eauto. }
-    {copy H3. nonEmptyStackTac H3. invertHyp. apply eraseTrmApp in H4. inv H4.  
-     exists H. exists T. split. constructor. split. simpl in *. econstructor.
-     eapply SPut; eauto. eassumption. econstructor. split. constructor. eauto. }
-    {copy H3. nonEmptyStackTac H3. invertHyp. apply eraseTrmApp in H4. inv H4.  
-     exists H. exists T. split. constructor. split. simpl in *. econstructor.
-     eapply SNew; eauto. eassumption. econstructor. split. constructor. eauto. }
-    {copy H3. nonEmptyStackTac H3. invertHyp. apply eraseTrmApp in H4. inv H4. 
-     exists h'. exists T. split. constructor. split. simpl in *. econstructor. 
-     eapply SSpec; eauto. eassumption. econstructor. split. constructor. eauto. }
-   }
-   }
-   Grab Existential Variables. rewrite lookupReplaceNeq; eauto. 
-Qed. 
-
+Ltac takeTStep :=
+  match goal with
+      |H:?T = ?x |- spec_multistep ?H (tUnion ?T ?T') ?H' ?T'' =>
+       rewrite H; unfoldTac; rewrite UnionSwap; 
+       econstructor;[eapply specStepChangeUnused; eassumption|idtac]; unfoldTac; 
+       rewrite <- UnionSwap                                          
+      |H:?T = ?x |- spec_multistep ?H (tUnion ?T ?T') ?H' ?T'' =>
+       rewrite H; unfoldTac; rewrite UnionSwap
+      |H:?T = ?x |- spec_multistep ?H (tUnion ?T ?T') ?H' ?T'' =>
+       rewrite H
+  end. 
 
 Theorem helper : forall H T H' T' ds ds' x M' TID,
                    heap_lookup x H = Some(sfull COMMIT ds SPEC TID M') ->
@@ -157,7 +19,7 @@ Theorem helper : forall H T H' T' ds ds' x M' TID,
                    spec_multistep H T H' T' ->
                    spec_multistep (replace x (sfull COMMIT ds COMMIT TID M') H) T
                                   (replace x (sfull COMMIT ds' COMMIT TID M') H') T'. 
-Proof. 
+Proof.  
   intros. genDeps{x; ds; ds'; TID; M'}. induction H2; intros. 
   {rewrite H1 in H0. inv H0. constructor. }
   {inversion H; subst. 
@@ -185,6 +47,102 @@ Proof.
   Grab Existential Variables. rewrite lookupReplaceNeq; eauto. 
 Qed. 
 
+Theorem writeFastForward : forall H T H' T' TID x M' E M'' s2 d s1' M,
+         heap_lookup x H = Some(sempty COMMIT) -> decompose M' E (put (fvar x) M'') ->
+         spec_multistep H (tUnion T (tSingleton(TID,unlocked nil,s2,M'))) H' 
+                        (tUnion T' (tSingleton(TID,unlocked(s1'++[wAct x M' E M'' d]),s2,M))) ->
+         exists H'' T'' ,
+           spec_multistep H (tUnion T (tSingleton(TID,unlocked nil,s2,M'))) H''
+                         (tUnion T'' (tSingleton(TID,unlocked [wAct x M' E M'' d],s2,fill E (ret unit)))) /\
+           spec_multistep H'' (tUnion T'' (tSingleton(TID,unlocked [wAct x M' E M'' d],s2,fill E (ret unit))))
+                          H' (tUnion T' (tSingleton(TID,unlocked(s1'++[wAct x M' E M'' d]),s2,M)))  /\
+           spec_multistep (replace x (sfull COMMIT nil COMMIT TID M'') H) T 
+                          (replace x (sfull COMMIT nil COMMIT TID M'')H'') T'' /\ 
+           heap_lookup x H'' = Some(sfull COMMIT nil SPEC TID M'').
+Proof.
+  intros. dependent induction H2. 
+  {apply UnionEqTID in x. invertHyp. inv H2. invertListNeq. }
+  {startIndCase. destructThread x1. exMid TID H9.
+   {apply UnionEqTID in H5. invertHyp. econstructor. econstructor. split. 
+    econstructor. eapply SPut; eauto. constructor. split. inv H3; try solve[falseDecomp].  
+    {inv H15. }
+    {copy d; copy d0. eapply uniqueCtxtDecomp in H3; eauto. invertHyp. inv H6. 
+     proofsEq d d0. rewrite H14 in H0. inv H0. eauto. }
+    {split. rewrite replaceOverwrite. constructor. erewrite HeapLookupReplace; eauto. }
+   } 
+   {apply UnionNeqTID in H5; auto. invertHyp. copy H3. eapply specStepEmptyIVar in H3; eauto.
+     Focus 2. rewrite H4. solveSet. left. invUnion. right; simpl. eauto. Focus 2. solveSet. 
+    copy H3. eapply IHspec_multistep in H3; eauto. invertHyp. econstructor. econstructor. split.
+    rewrite H11; unfoldTac; rewrite UnionSwap; econstructor. eapply specStepChangeUnused. 
+    eauto. unfoldTac. rewrite UnionSwap. eassumption. split; eauto. split; eauto. 
+    Focus 2. rewrite H4. rewrite UnionSubtract. unfoldTac. rewrite UnionSwap. eauto.
+    rewrite H11. clear H11 H4. inv H5. 
+    {econstructor. eapply SBasicStep;eauto.  eauto. }
+    {econstructor. eapply SFork; eauto. eauto. }
+    {varsEq x3 x0. heapsDisagree. econstructor. eapply SGet; eauto.
+     erewrite lookupReplaceNeq; eauto. rewrite lookupReplaceSwitch; eauto. }
+    {varsEq x3 x0. erewrite HeapLookupReplace in H12; eauto. inv H12. econstructor. 
+     eapply SPut. rewrite lookupReplaceNeq; eauto. auto. rewrite lookupReplaceSwitch. 
+     eauto. auto. }
+    {varsEq x3 x0. heapsDisagree. econstructor. eapply SNew; eauto. 
+     erewrite extendReplaceSwitch; eauto. }
+    {econstructor. eapply SSpec; eauto. eauto. }
+   }
+  }
+  Grab Existential Variables. rewrite lookupReplaceNeq; eauto. 
+Qed. 
+
+Theorem writeSimPureSteps : forall H T H' T' TID x M' E M'' d N N' N'' s2 s1' ds ds',
+       eraseTrm s1' N' N'' -> 
+       heap_lookup x H = Some(sfull COMMIT ds SPEC TID M'') ->       
+       heap_lookup x H' = Some(sfull COMMIT ds' SPEC TID M'') -> 
+       spec_multistep H (tUnion T (tSingleton(TID,unlocked[wAct x M' E M'' d],s2,N))) H'
+                      (tUnion T' (tSingleton(TID,unlocked(s1'++[wAct x M' E M'' d]),s2,N'))) ->
+       exists H'' T'',
+         spec_multistep H (tUnion T (tSingleton(TID,unlocked[wAct x M' E M'' d],s2,N))) 
+                        H'' (tUnion T'' (tSingleton(TID,unlocked[wAct x M' E M'' d],s2,N''))) /\
+         spec_multistep H'' (tUnion T'' (tSingleton(TID,unlocked[wAct x M' E M'' d],s2,N''))) 
+                        H' (tUnion T' (tSingleton(TID,unlocked(s1'++[wAct x M' E M'' d]),s2,N'))) /\
+         exists ds'',
+         spec_multistep (replace x (sfull COMMIT ds COMMIT TID M'') H) T 
+                        (replace x (sfull COMMIT ds'' COMMIT TID M'')H'') T'' /\
+         heap_lookup x H'' = Some(sfull COMMIT ds'' SPEC TID M'').
+Proof.
+  intros. genDeps{N'';ds; ds'}. dependent induction H3; intros.
+  {apply UnionEqTID in x. invertHyp. inv H. destruct s1'; inv H5. inv H0; try invertListNeq. 
+   rewrite H2 in H1. inv H1. repeat econstructor. eauto. invertListNeq. }
+  {startIndCase. destructThread x1. exMid TID H10. 
+   {apply UnionEqTID in H6. invertHyp. inv H0. 
+    {eapply IHspec_multistep in H1;[idtac|eauto|eauto|eauto|eauto|eauto|eauto]. invertHyp. 
+     econstructor. econstructor. split. econstructor. eapply SBasicStep; eauto. eassumption. 
+     split. eassumption. econstructor. split. eassumption. eassumption. }
+    {copy H3. nonEmptyStackTac H3. invertHyp. apply eraseTrmApp in H4. inv H4. exists h'. 
+     exists T. split. constructor. split. simpl in *. econstructor. eapply SFork; eauto. 
+     eassumption. econstructor. split. constructor. eauto. }
+    {copy H3. nonEmptyStackTac H3. invertHyp. apply eraseTrmApp in H4. inv H4. 
+     exists H. exists T. split. constructor. split. simpl in *. econstructor. 
+     eapply SGet; eauto. eassumption. econstructor. split. constructor. eauto. }
+    {copy H3. nonEmptyStackTac H3. invertHyp. apply eraseTrmApp in H4. inv H4.  
+     exists H. exists T. split. constructor. split. simpl in *. econstructor.
+     eapply SPut; eauto. eassumption. econstructor. split. constructor. eauto. }
+    {copy H3. nonEmptyStackTac H3. invertHyp. apply eraseTrmApp in H4. inv H4.  
+     exists H. exists T. split. constructor. split. simpl in *. econstructor.
+     eapply SNew; eauto. eassumption. econstructor. split. constructor. eauto. }
+    {copy H3. nonEmptyStackTac H3. invertHyp. apply eraseTrmApp in H4. inv H4. 
+     exists h'. exists T. split. constructor. split. simpl in *. econstructor. 
+     eapply SSpec; eauto. eassumption. econstructor. split. constructor. eauto. }
+   }
+   {copy H0. eapply specStepFullIVar in H0; eauto. invertHyp. apply UnionNeqTID in x. invertHyp. 
+    copy H12. eapply IHspec_multistep in H12; eauto. invertHyp. econstructor. econstructor. 
+    split. rewrite H13. unfoldTac; rewrite UnionSwap. econstructor. 
+    eapply specStepChangeUnused. eauto. unfoldTac. rewrite UnionSwap. eassumption. 
+    split; eauto. econstructor. split. eapply spec_multi_trans. Focus 2. eassumption.  
+    eapply helper. eauto. eauto. rewrite H13. econstructor. eapply specStepChangeUnused. 
+    eauto. constructor. eauto. rewrite H0. rewrite UnionSubtract. unfoldTac. 
+    rewrite UnionSwap. eauto. auto. }
+  }
+Qed. 
+
 Theorem writeSimActionSteps : forall H T H' T' TID x M' E M'' d N N' H'' T'' N'' s2 s1 s1' ds ds' a,
                                 eraseTrm (s1'++[a]) N' N'' ->
        heap_lookup x H = Some(sfull COMMIT ds SPEC TID M'') ->       
@@ -203,62 +161,55 @@ Proof.
    replace[a;wAct x0 M' E M'' d] with ([a]++[wAct x0 M' E M'' d]) in H6; auto. 
    rewrite app_assoc in H6. apply app_inj_tail in H6. invertHyp. rewrite H2 in H1. 
    inv H1. constructor. }
-  {copy x. copy H1. apply specStepSingleton in H1. invertHyp. unfoldSetEq H6.
-   assert(tIn(tUnion T0(tSingleton x1)) x1). apply Union_intror. constructor. 
-   apply H1 in H6. inv H6.  
-   {copy H9. apply pullOut in H9. rewrite H9. clear H9. copy H7. destruct x1. destruct p.  
-    destruct p. copy H9. eapply specStepFullIVar in H9; eauto. inv H9. 
-    {eapply spec_multi_trans. eapply spec_multi_unused. eapply helper. eauto. eapply H11. 
-     eapply smulti_step. eapply specStepChangeUnused. eassumption. constructor. 
-     eapply IHspec_multistep in H11; eauto. eapply spec_multi_trans. eassumption. 
-     apply pullOut in H6. rewrite H6. unfoldTac. rewrite UnionSwap. econstructor. 
-     eapply specStepChangeUnused. eauto. unfoldTac. rewrite <- UnionSwap. 
-     rewrite subtractSingle. constructor. proveUnionEq x. }
-   }
-   {inv H9. apply UnionEqTID in x. invertHyp. inv H6. 
-    inversion H7; subst; unfoldTac; invertHyp; invThreadEq.  
+  {startIndCase. destructThread x1. exMid TID H11. 
+   {apply UnionEqTID in H7. invertHyp. inversion H1; subst. 
     {copy H3. eapply stackNonNil in H3. destruct s1. exfalso. apply H3. auto. 
      econstructor. eapply SBasicStep; eauto. constructor. eapply IHspec_multistep; eauto. 
      eapply spec_multi_trans. eassumption. econstructor. eapply SBasicStep; eauto. constructor. 
-     eauto. intros c. subst. apply eraseTrmApp in H0. inv H0; inv H10; falseDecomp. }
-    {econstructor. eapply SFork; eauto. unfoldTac. rewrite coupleUnion. rewrite <- Union_associative. 
+     eauto. intros c. subst. apply eraseTrmApp in H0. inv H0; inv H16; falseDecomp. }
+    {econstructor. eapply SFork; eauto. unfoldTac. rewrite coupleUnion. rewrite Union_associative. 
      rewrite <- UnionSwap. eapply IHspec_multistep; eauto. Focus 2. 
-     rewrite Union_associative. rewrite <- coupleUnion. rewrite couple_swap. 
+     rewrite <- Union_associative. rewrite <- coupleUnion. rewrite couple_swap. 
      unfold numForks. simpl. simpl. eauto. rewrite numForksDistribute. simpl. rewrite <- plus_assoc. 
      rewrite <- plus_comm. simpl. rewrite plus_comm. reflexivity. eapply spec_multi_trans. 
-     eassumption. econstructor. eapply SFork; eauto. rewrite Union_associative. rewrite <- coupleUnion. 
+     eassumption. econstructor. eapply SFork; eauto. rewrite <- Union_associative. rewrite <- coupleUnion. 
      rewrite couple_swap. simpl. rewrite numForksDistribute. simpl. rewrite <- plus_assoc. 
      rewrite plus_comm. simpl. rewrite plus_comm. constructor. }
-    {destruct(beq_nat x x0) eqn:eq. 
-     {apply beq_nat_true in eq. subst. rewrite H5 in H10. inv H10. econstructor. 
-      eapply SGet with(x:=x0); eauto. erewrite HeapLookupReplace; eauto. lookupTac. 
+    {varsEq x0 x1. 
+     {rewrite H5 in H16. inv H16. econstructor. eapply SGet with(x:=x1); eauto. 
+      erewrite HeapLookupReplace; eauto. lookupTac. 
       eapply IHspec_multistep in H6; eauto. rewrite replaceOverwrite. rewrite replaceOverwrite in H6. 
-      eassumption. eapply spec_multi_trans. eassumption. econstructor. eapply SGet with(x:=x0); eauto. 
+      eassumption. eapply spec_multi_trans. eassumption. econstructor. eapply SGet with(x:=x1); eauto. 
       constructor. simpl. eauto. }
-     {apply beq_nat_false in eq. apply neqSym in eq. lookupTac. eapply IHspec_multistep in H6; eauto. 
-      econstructor. eapply SGet with(x:=x); auto. rewrite lookupReplaceNeq; eauto. 
+     {lookupTac. eapply IHspec_multistep in H7; eauto. 
+      econstructor. eapply SGet with(x:=x1); auto. rewrite lookupReplaceNeq; eauto. 
       rewrite lookupReplaceSwitch; auto. eassumption. eapply spec_multi_trans. eassumption. 
-      econstructor. eapply SGet with(x:=x); eauto. constructor. simpl. eauto. }
+      econstructor. eapply SGet with(x:=x1); eauto. constructor. simpl. eauto. }
     }
-    {destruct (beq_nat x x0) eqn:eq. apply beq_nat_true in eq. subst. rewrite H10 in H5. 
-     inv H5. apply beq_nat_false in eq. apply neqSym in eq. lookupTac.
-     eapply IHspec_multistep in H6; eauto. econstructor. eapply SPut with(x:=x). 
-     rewrite lookupReplaceNeq; eauto. auto. rewrite lookupReplaceSwitch; auto. simpl. 
-     eassumption. eapply spec_multi_trans. eassumption. econstructor. eapply SPut with(x:=x). 
-     eauto. auto. constructor. simpl. reflexivity. }
-    {destruct (beq_nat x x0) eqn:eq. apply beq_nat_true in eq. subst. copy p. rewrite H6 in H5. 
-     inv H5. apply beq_nat_false in eq. apply neqSym in eq. lookupTac.
-     eapply IHspec_multistep in H6; eauto. econstructor. eapply SNew with(x:=x). 
-     auto. erewrite extendReplaceSwitch; eauto. eapply spec_multi_trans. eassumption. 
-     econstructor. eapply SNew with(x:=x); eauto. constructor. simpl. auto. }
-    {econstructor. eapply SSpec; eauto. unfoldTac. rewrite coupleUnion. rewrite <- Union_associative. 
-     rewrite <- UnionSwap. eapply IHspec_multistep; eauto. Focus 2. rewrite Union_associative. 
+    {varsEq x0 x1. heapsDisagree. lookupTac. eapply IHspec_multistep in H7; eauto. 
+     econstructor. eapply SPut with(x:=x1). rewrite lookupReplaceNeq; eauto. auto. 
+     rewrite lookupReplaceSwitch; auto. simpl. eassumption. eapply spec_multi_trans.
+     eassumption. econstructor. eapply SPut with(x:=x1).  eauto. auto. 
+     constructor. simpl. reflexivity. }
+    {varsEq x0 x1. heapsDisagree. lookupTac. eapply IHspec_multistep in H7; eauto. 
+     econstructor. eapply SNew with(x:=x1). auto. erewrite extendReplaceSwitch; eauto.
+     eapply spec_multi_trans. eassumption. econstructor. eapply SNew with(x:=x1); eauto. 
+     constructor. simpl. auto. }
+    {econstructor. eapply SSpec; eauto. unfoldTac. rewrite coupleUnion. rewrite Union_associative. 
+     rewrite <- UnionSwap. eapply IHspec_multistep; eauto. Focus 2. rewrite <- Union_associative. 
      rewrite <- coupleUnion.  rewrite couple_swap. reflexivity. eapply spec_multi_trans. 
-     eassumption. econstructor. eapply SSpec; eauto. rewrite Union_associative. rewrite <- coupleUnion. 
+     eassumption. econstructor. eapply SSpec; eauto. rewrite <- Union_associative. rewrite <- coupleUnion. 
      rewrite couple_swap. constructor. }
    }
+   {apply UnionNeqTID in H7; auto. copy H1. eapply specStepFullIVar in H1; eauto. invertHyp. 
+    copy H13. eapply IHspec_multistep in H13; eauto. eapply spec_multi_trans. Focus 2. eassumption. 
+    eapply helper; eauto. unfoldTac. rewrite UnionSwap. rewrite H14. rewrite UnionSwap. 
+    econstructor. eapply specStepChangeUnused. eauto. constructor. eapply spec_multi_trans. 
+    eassumption. rewrite H14. unfoldTac. rewrite UnionSwap. econstructor. 
+    eapply specStepChangeUnused; eauto. unfoldTac. rewrite UnionSwap. constructor. 
+    rewrite H1. rewrite UnionSubtract. unfoldTac. rewrite UnionSwap; eauto. }
   }
-  Grab Existential Variables. rewrite lookupReplaceNeq; eauto. 
+  Grab Existential Variables. rewrite lookupReplaceNeq; eauto.
 Qed. 
 
 
